theories/Stlc/Predicates.v
@@ -36,8 +36,9 @@ From iris Require
   bi.derived_connectives
   bi.interface
   proofmode.tactics.
+From stdpp Require Import
+  base.
 From Em Require Import
-  Context
   Environment
   Prelude
   Stlc.Alloc
@@ -54,10 +55,10 @@ Import world.notations.
 #[local] Arguments step : simpl never.
 #[local] Arguments thick : simpl never.
 
-#[local] Notation "Q [ ζ ]" :=
-  (_4 Q ζ)
-    (at level 8, left associativity,
-      format "Q [ ζ ]") : box_scope.
+(* #[local] Notation "Q [ ζ ]" := *)
+(*   (_4 Q ζ) *)
+(*     (at level 8, left associativity, *)
+(*       format "Q [ ζ ]") : box_scope. *)
 
 Module Pred.
   #[local] Notation Ėxp := (Sem Exp).
@@ -69,9 +70,24 @@ Module Pred.
     Assignment w -> Prop.
   Bind Scope pred_scope with Pred.
 
-  Section RewriteRelations.
+  Section Definitions.
 
-    Import iris.bi.interface.
+    Definition eqₚ {T : TYPE} {A : Type} {instTA : Inst T A} :
+      ⊧ T ⇢ T ⇢ Pred :=
+      fun w t1 t2 ι => inst t1 ι = inst t2 ι.
+    #[global] Arguments eqₚ {T A _} [w] _ _ _/.
+
+    Definition TPB : ⊧ Ėnv ⇢ Const Exp ⇢ Ṫy ⇢ Ėxp ⇢ Pred :=
+      fun w G e t ee ι => inst G ι |-- e ∷ inst t ι ~> inst ee ι.
+    #[global] Arguments TPB [w] G e t ee ι/.
+
+    #[export] Instance persist_pred : Persistent Pred :=
+      fun Θ w1 P w2 θ ι2 => P (inst θ ι2).
+    #[global] Arguments persist_pred Θ [w] _ [w1] _ _ /.
+
+  End Definitions.
+
+  Section RewriteRelations.
 
     Context {w : World}.
 
@@ -107,50 +123,6 @@ Module Pred.
   #[global] Arguments bientails {w} (_ _)%P.
   #[global] Arguments entails {w} (_ _)%P.
 
-  Section Definitions.
-    Import World.notations.
-
-    Definition Falseₚ : ⊧ Pred :=
-      fun w _ => Logic.False.
-    Definition Trueₚ : ⊧ Pred :=
-      fun w _ => Logic.True.
-    Definition iffₚ : ⊧ Pred ⇢ Pred ⇢ Pred :=
-      fun w P Q ι => P ι <-> Q ι.
-    Definition implₚ : ⊧ Pred ⇢ Pred ⇢ Pred :=
-      fun w P Q ι => P ι -> Q ι.
-    Definition andₚ : ⊧ Pred ⇢ Pred ⇢ Pred :=
-      fun w P Q ι => P ι /\ Q ι.
-    Definition orₚ : ⊧ Pred ⇢ Pred ⇢ Pred :=
-      fun w P Q ι => P ι \/ Q ι.
-    #[global] Arguments andₚ {_} (_ _)%P _/.
-    #[global] Arguments orₚ {_} (_ _)%P _/.
-    #[global] Arguments iffₚ {_} (_ _)%P _/.
-    #[global] Arguments implₚ {_} (_ _)%P _/.
-    #[global] Arguments Trueₚ {_} _/.
-    #[global] Arguments Falseₚ {_} _/.
-
-    Definition eqₚ {T : TYPE} {A : Type} {instTA : Inst T A} :
-      ⊧ T ⇢ T ⇢ Pred :=
-      fun w t1 t2 ι => inst t1 ι = inst t2 ι.
-    #[global] Arguments eqₚ {T A _} [w] _ _ _/.
-
-    (* #[universes(polymorphic)]  *)Definition Forall {I : Type} {w} :
-      (I -> Pred w) -> Pred w := fun A ι => forall i : I, A i ι.
-    (* #[universes(polymorphic)]  *)Definition Exists {I : Type} {w} :
-      (I -> Pred w) -> Pred w := fun A ι => exists i : I, A i ι.
-    #[global] Arguments Forall {I w} A%P ι/.
-    #[global] Arguments Exists {I w} A%P ι/.
-
-    Definition TPB : ⊧ Ėnv ⇢ Const Exp ⇢ Ṫy ⇢ Ėxp ⇢ Pred :=
-      fun w G e t ee ι => inst G ι |-- e ∷ inst t ι ~> inst ee ι.
-    #[global] Arguments TPB [w] G e t ee ι/.
-
-    #[export] Instance persist_pred : Persistent Pred :=
-      fun Θ w1 P w2 θ ι2 => P (inst θ ι2).
-    #[global] Arguments persist_pred Θ [w] _ [w1] _ _ /.
-
-  End Definitions.
-
   Module Import proofmode.
 
     Import iris.bi.interface.
@@ -167,12 +139,6 @@ Module Pred.
     #[export] Instance ofe_dist_pred {w} : ofe.Dist (Pred w) :=
       ofe.discrete_dist.
 
-    Definition bimixin_pred {w : World} :
-      BiMixin entails empₚ (fun P _ => P) andₚ orₚ implₚ
-        (fun A => @Pred.Forall A w) (fun A => @Pred.Exists A w)
-        sepₚ wandₚ persistently.
-    Proof. firstorder. Qed.
-
     (* Iris defines [bi_later_mixin_id] for BI algebras without later. However,
        the identity function as later still causes some later-specific
        typeclasses to be picked. We just define our own trivial modality and
@@ -180,17 +146,25 @@ Module Pred.
     Variant later {w} (P : Pred w) (ι : Assignment w) : Prop :=
       MkLater : P ι -> later P ι.
 
-    Definition bilatermixin_pred {w} :
-      BiLaterMixin entails (fun P _ => P) orₚ implₚ
-        (fun A => @Pred.Forall A w) (fun A => @Pred.Exists A w)
-        sepₚ persistently later.
-    Proof. firstorder. Qed.
-
-    Canonical bi_pred {w : World} : bi :=
-      {| bi_car            := Pred w;
-         bi_bi_mixin       := bimixin_pred;
-         bi_bi_later_mixin := bilatermixin_pred;
-      |}.
+    Canonical bi_pred {w : World} : bi.
+    Proof.
+      refine
+        {| bi_car := Pred w;
+           bi_entails := entails;
+           bi_emp := empₚ;
+           bi_pure P _ := P;
+           bi_and P Q ι := P ι /\ Q ι;
+           bi_or P Q ι := P ι \/ Q ι;
+           bi_impl P Q ι := P ι -> Q ι;
+           bi_forall A f ι := forall a, f a ι;
+           bi_exist A f ι := exists a, f a ι;
+           bi_sep := sepₚ;
+           bi_wand := wandₚ;
+           bi_persistently := persistently;
+           bi_later := later;
+        |}.
+      all: abstract firstorder.
+    Defined.
 
     #[export] Instance persistent_pred {w} {P : Pred w} :
       derived_connectives.Persistent P.
@@ -214,7 +188,8 @@ Module Pred.
       (@equiv (bi_car (@bi_pred _)) (@pred_equiv _))
         (only parsing).
 
-    Infix "⊢ₚ" := (entails) (at level 95).
+    Notation "P ⊢ₚ Q" := (@bi_entails (@bi_pred _) P%P Q%P) (at level 95).
+    Notation "(⊢ₚ)" := (@bi_entails (@bi_pred _)) (only parsing).
 
     Notation "⊤ₚ" := (@bi_pure (@bi_pred _) True) : pred_scope.
     Notation "⊥ₚ" := (@bi_pure (@bi_pred _) False) : pred_scope.
@@ -234,48 +209,80 @@ Module Pred.
       (at level 200, x binder, y binder, right associativity,
         format "'[ ' '[ ' ∃ₚ  x .. y ']' ,  '/' P ']'") : pred_scope.
 
-    Notation "'Fun' x => b" :=
-      (fun w ζ x => b%P w ζ)
-        (x binder, at level 100, only parsing) : pred_scope.
-
     Notation "G |--ₚ E ; T ~> EE" :=
       (TPB G E T EE) (at level 70, no associativity) : pred_scope.
 
   End notations.
 
+  Lemma bientails_unfold [w] (P Q : Pred w) :
+    (P ⊣⊢ₚ Q) <-> forall ι, P ι <-> Q ι.
+  Proof. firstorder. Qed.
+  Lemma entails_unfold [w] (P Q : Pred w) :
+    (P ⊢ₚ Q) <-> forall ι, P ι -> Q ι.
+  Proof. firstorder. Qed.
+  Lemma sep_unfold w (P Q : Pred w) :
+    ∀ ι, interface.bi_sep P Q ι ↔ (P ι /\ Q ι).
+  Proof. firstorder. Qed.
+  Lemma wand_unfold w (P Q : Pred w) :
+    ∀ ι, interface.bi_wand P Q ι ↔ (P ι → Q ι).
+  Proof. firstorder. Qed.
+  Lemma intuitionistically_unfold w (P : Pred w) :
+    ∀ ι, @derived_connectives.bi_intuitionistically _ P ι <-> P ι.
+  Proof. firstorder. Qed.
+
+  Create HintDb punfold.
+  #[export] Hint Rewrite bientails_unfold entails_unfold sep_unfold wand_unfold
+    intuitionistically_unfold
+    (@inst_persist Ėnv Env _ _ _)
+    (@inst_persist Ėxp Exp _ _ _)
+    (@inst_persist Ṫy Ty _ _ _)
+    (@inst_lift Ėnv Env _ _ _)
+    (@inst_lift Ėxp Exp _ _ _)
+    (@inst_lift Ṫy Ty _ _ _)
+    (@inst_thin Sub _ Sub.lk_thin_sub)
+    @inst_refl @inst_trans @inst_insert
+    @Sem.inst_pure
+    @ėxp.inst_var @ėxp.inst_true @ėxp.inst_false @ėxp.inst_ifte @ėxp.inst_absu
+    @ėxp.inst_abst @ėxp.inst_app : punfold.
+
+  Ltac punfold_connectives :=
+    change (@interface.bi_and (@bi_pred _) ?P ?Q ?ι) with (P ι /\ Q ι) in *;
+    change (@interface.bi_or (@bi_pred _) ?P ?Q ?ι) with (P ι \/ Q ι) in *;
+    change (@interface.bi_impl (@bi_pred _) ?P ?Q ?ι) with (P ι -> Q ι) in *;
+    change (@derived_connectives.bi_iff (@bi_pred _) ?P ?Q ?ι) with (iff (P ι) (Q ι)) in *;
+    change (@interface.bi_pure (@bi_pred _) ?P _) with P in *;
+    change (@interface.bi_forall (@bi_pred _) ?A ?P) with (fun ι => forall a : A, P a ι) in *;
+    change (@interface.bi_exist (@bi_pred _) ?A ?P) with (fun ι => exists a : A, P a ι) in *;
+    change (@persist Pred persist_pred _ _ ?P _ ?θ ?ι) with (P (inst θ ι)) in *;
+    try progress (cbn beta).
+
   Ltac pred_unfold :=
     repeat
-      (change (@interface.bi_and (@bi_pred ?w)) with (@andₚ w) in *;
-       change (@interface.bi_or (@bi_pred ?w)) with (@orₚ w) in *;
-       change (@interface.bi_impl (@bi_pred ?w)) with (@implₚ w) in *;
-       change (@derived_connectives.bi_iff (@bi_pred ?w)) with (@iffₚ w) in *;
-       change (@interface.bi_pure (@bi_pred ?w)) with (fun (P : Prop) (ι : Assignment w) => P) in *;
-       change (@interface.bi_forall (@bi_pred ?w)) with (fun A => @Forall A w) in *;
-       change (@interface.bi_exist (@bi_pred ?w)) with (fun A => @Exists A w) in *;
-       change (@persist Pred persist_pred _ _ ?P _ ?θ ?ι) with (P (inst θ ι)) in *;
-       cbn [andₚ orₚ implₚ iffₚ Forall Exists eqₚ TPB inst inst_ty inst_env] in *;
-
-       repeat rewrite ?inst_persist, ?inst_lift, ?inst_refl, ?inst_trans,
-         ?inst_insert, ?ėxp.inst_var, ?ėxp.inst_true, ?ėxp.inst_false,
-         ?ėxp.inst_absu, ?ėxp.inst_abst, ?ėxp.inst_app, ?ėxp.inst_ifte in *;
-       repeat
+      (punfold_connectives;
+       try rewrite_db punfold; auto 1 with typeclass_instances;
+       cbn [eqₚ TPB inst inst_ty inst_env] in *;
+       (* repeat rewrite ?inst_persist, ?inst_lift, ?inst_refl, ?inst_trans, *)
+       (*   ?inst_insert, ?ėxp.inst_var, ?ėxp.inst_true, ?ėxp.inst_false, *)
+       (*   ?ėxp.inst_absu, ?ėxp.inst_abst, ?ėxp.inst_app, ?ėxp.inst_ifte in *; *)
+       try
          match goal with
+         | |- forall ι : Assignment _, _ =>
+             let ι := fresh "ι" in
+             intro ι; pred_unfold;
+             first [clear ι | revert ι]
          | |- @interface.bi_emp_valid (@bi_pred _) _ => constructor; intros ι _; cbn
          | |- @interface.bi_entails (@bi_pred _) _ _ => constructor; intros ι; cbn
-         | H: context[@inst ?AT ?A ?I ?w ?x ?ι] |- _ =>
-             is_var x; generalize dependent x; intro x;
-             generalize (@inst AT A I w x ι);
-             clear x; intro x; intros; subst
+         (* | H: context[@inst ?AT ?A ?I ?w ?x ?ι] |- _ => *)
+         (*     is_var x; generalize (@inst AT A I w x ι); *)
+         (*     clear x; intro x; subst *)
          | |- context[@inst ?AT ?A ?I ?w ?x ?ι] =>
-             is_var x; generalize dependent x; intro x;
-             generalize (@inst AT A I w x ι);
-             clear x; intro x; intros; subst
+             is_var x; generalize (@inst AT A I w x ι);
+             clear x; intro x; subst
          end).
 
   Section Lemmas.
 
     Import iris.bi.interface.
-    Import stdpp.base.
 
     Create HintDb obligation.
     #[local] Hint Rewrite @inst_refl @inst_trans : obligation.
@@ -285,8 +292,8 @@ Module Pred.
       repeat (autorewrite with obligation in *; cbn in *; intros; subst; pred_unfold);
       repeat
         (match goal with
-         (* | H: _ ⊢ₚ _ |- _ => destruct H as [H] *)
-         (* | H: _ ⊣⊢ₚ _ |- _ => destruct H as [H] *)
+         | H: _ ⊢ₚ _ |- _ => destruct H as [H]
+         | H: _ ⊣⊢ₚ _ |- _ => destruct H as [H]
          | H: forall (H : ?A), _, a : ?A |- _ =>
            specialize (H a); autorewrite with obligation in H; cbn in H
          | |- (forall _ : ?A, _) <-> (forall _ : ?A, _) =>
@@ -299,52 +306,15 @@ Module Pred.
       try easy; try (intuition; fail); try (intuition congruence; fail).
     #[local] Obligation Tactic := obligation.
 
-    Lemma entails_in [w] (P Q : Pred w) :
-      (P ⊢ₚ Q) <-> forall ι, P ι -> Q ι.
-    Proof. split; [intros []|]; obligation. Qed.
-    Lemma equiv_in [w] (P Q : Pred w) :
-      (P ⊣⊢ₚ Q) <-> forall ι, P ι <-> Q ι.
-    Proof. split; [intros []|]; obligation. Qed.
-
-    #[local] Hint Rewrite entails_in equiv_in : obligation.
     #[local] Hint Rewrite <- @tactics.forall_and_distr : obligation.
 
-    #[export,program] Instance proper_iff {w} :
-      Proper ((⊣⊢ₚ) ==> (⊣⊢ₚ) ==> (⊣⊢ₚ)) (@iffₚ w).
-    #[export,program] Instance proper_impl_bientails {w} :
-      Proper ((⊣⊢ₚ) ==> (⊣⊢ₚ) ==> (⊣⊢ₚ)) (@implₚ w).
-    #[export,program] Instance proper_impl_entails {w} :
-      Proper (entails --> entails ==> entails) (@implₚ w).
-    #[export,program] Instance proper_and_bientails {w} :
-      Proper ((⊣⊢ₚ) ==> (⊣⊢ₚ) ==> (⊣⊢ₚ)) (@andₚ w).
-    #[export,program] Instance proper_and_entails {w} :
-      Proper (entails ==> entails ==> entails) (@andₚ w).
-    #[export,program] Instance proper_or_bientails {w} :
-      Proper ((⊣⊢ₚ) ==> (⊣⊢ₚ) ==> (⊣⊢ₚ)) (@orₚ w).
-    #[export,program] Instance proper_or_entails {w} :
-      Proper (entails ==> entails ==> entails) (@orₚ w).
-    #[export,program] Instance proper_forall_bientails {I w} :
-      Proper (pointwise_relation I (⊣⊢ₚ) ==> (⊣⊢ₚ)) (@Pred.Forall I w).
-    #[export,program] Instance proper_exists_bientails {I w} :
-      Proper (pointwise_relation I (⊣⊢ₚ) ==> (⊣⊢ₚ)) (@Pred.Exists I w).
-    #[export,program] Instance proper_persist_bientails {Θ w} :
+    #[export] Instance proper_persist_bientails {Θ w} :
       Proper ((⊣⊢ₚ) ==> forall_relation (fun _ => eq ==> (⊣⊢ₚ)))
-        (@persist Pred persist_pred Θ w).
+      (@persist Pred persist_pred Θ w).
+    Proof. obligation. Qed.
 
     Lemma split_bientails {w} (P Q : Pred w) :
       (P ⊣⊢ₚ Q) <-> (P ⊢ₚ Q) /\ (Q ⊢ₚ P).
-    Proof. obligation. Qed.
-    Lemma and_left1 {w} {P Q R : Pred w} : P ⊢ₚ R -> P /\ₚ Q ⊢ₚ R.
-    Proof. obligation. Qed.
-    Lemma and_left2 {w} {P Q R : Pred w} : Q ⊢ₚ R -> P /\ₚ Q ⊢ₚ R.
-    Proof. obligation. Qed.
-    Lemma and_right {w} {P Q R : Pred w} : P ⊢ₚ Q -> P ⊢ₚ R -> P ⊢ₚ Q /\ₚ R.
-    Proof. obligation. Qed.
-    Lemma or_right1 {w} {P Q : Pred w} : P ⊢ₚ P \/ₚ Q.
-    Proof. obligation. Qed.
-    Lemma or_right2 {w} {P Q : Pred w} : Q ⊢ₚ P \/ₚ Q.
-    Proof. obligation. Qed.
-    Lemma or_left {w} {P Q R : Pred w} : P ⊢ₚ R -> Q ⊢ₚ R -> P \/ₚ Q ⊢ₚ R.
     Proof. obligation. Qed.
     Lemma impl_and_adjoint {w} (P Q R : Pred w) : (P /\ₚ Q ⊢ₚ R) <-> (P ⊢ₚ Q ->ₚ R).
     Proof. obligation. Qed.
@@ -366,21 +336,21 @@ Module Pred.
     Proof. obligation. Qed.
     Lemma impl_false_l {w} (P : Pred w) : ⊥ₚ ->ₚ P ⊣⊢ₚ ⊤ₚ.
     Proof. obligation. Qed.
-    Lemma false_l {w} (P : Pred w) : ⊥ₚ ⊢ₚ P.
-    Proof. obligation. Qed.
-    Lemma true_r {w} (P : Pred w) : P ⊢ₚ ⊤ₚ.
-    Proof. obligation. Qed.
-    Lemma impl_forget {w} (P Q R : Pred w) : P ⊢ₚ R -> P ⊢ₚ (Q ->ₚ R).
-    Proof. obligation. Qed.
+    (* Lemma false_l {w} (P : Pred w) : ⊥ₚ ⊢ₚ P. *)
+    (* Proof. obligation. Qed. *)
+    (* Lemma true_r {w} (P : Pred w) : P ⊢ₚ ⊤ₚ. *)
+    (* Proof. obligation. Qed. *)
+    (* Lemma impl_forget {w} (P Q R : Pred w) : P ⊢ₚ R -> P ⊢ₚ (Q ->ₚ R). *)
+    (* Proof. obligation. Qed. *)
     Lemma impl_and [w] (P Q R : Pred w) : ((P /\ₚ Q) ->ₚ R) ⊣⊢ₚ (P ->ₚ Q ->ₚ R).
     Proof. obligation. Qed.
 
-    Lemma forall_l {I : Type} {w} (P : I -> Pred w) Q :
-      (exists x : I, P x ⊢ₚ Q) -> (∀ x : I, P x)%I ⊢ₚ Q.
-    Proof. obligation. firstorder. Qed.
-    Lemma forall_r {I : Type} {w} P (Q : I -> Pred w) :
-      (P ⊢ₚ (∀ₚ x : I, Q x)) <-> (forall x : I, P ⊢ₚ Q x).
-    Proof. obligation. firstorder. Qed.
+    (* Lemma forall_l {I : Type} {w} (P : I -> Pred w) Q : *)
+    (*   (exists x : I, P x ⊢ₚ Q) -> (∀ x : I, P x)%I ⊢ₚ Q. *)
+    (* Proof. obligation. firstorder. Qed. *)
+    (* Lemma forall_r {I : Type} {w} P (Q : I -> Pred w) : *)
+    (*   (P ⊢ₚ (∀ₚ x : I, Q x)) <-> (forall x : I, P ⊢ₚ Q x). *)
+    (* Proof. obligation. firstorder. Qed. *)
 
     Lemma exists_l {I : Type} {w} (P : I -> Pred w) (Q : Pred w) :
       (forall x : I, P x ⊢ₚ Q) -> (∃ₚ x : I, P x) ⊢ₚ Q.
@@ -392,7 +362,7 @@ Module Pred.
 
     Lemma wand_is_impl [w] (P Q : Pred w) :
       (P -∗ Q)%I ⊣⊢ₚ (P ->ₚ Q).
-    Proof. firstorder. Qed.
+    Proof. obligation. Qed.
 
     Lemma pApply {w} {P Q R : Pred w} :
       P ⊢ₚ Q -> Q ⊢ₚ R -> P ⊢ₚ R.
@@ -437,16 +407,23 @@ Module Pred.
       [w] (a1 a2 : AT w) (b1 b2 : BT w) :
       (a1,b1) =ₚ (a2,b2) ⊣⊢ₚ ((a1 =ₚ a2) /\ₚ (b1 =ₚ b2)).
     Proof.
-      constructor. pred_unfold. intros ι; cbn. split.
+      pred_unfold. intros ι; cbn. split.
       - now injection 1.
       - intros []. now f_equal.
     Qed.
 
     Section Persist.
 
-      Import World.notations.
+      Lemma persist_eq {T : TYPE} {persR : Persistence.Persistent T}
+        {A : Type} {instTA : Inst T A} {instPersistTA : InstPersist T A}
+        {Θ : SUB} {w0 w1} (θ : Θ w0 w1) (t1 t2 : T w0) :
+        persist (t1 =ₚ t2) θ ⊣⊢ₚ persist t1 θ =ₚ persist t2 θ.
+      Proof.
+        pred_unfold. unfold persist, persist_pred. intros ι.
+        now rewrite !inst_persist.
+      Qed.
 
-      Context {Θ : ACC}.
+      Context {Θ : SUB}.
 
       (* We could define a PersistLaws instance for the Pred type, but that's
          requires functional extensionality. Instead, we provide similar
@@ -466,23 +443,14 @@ Module Pred.
         persist (P ->ₚ Q) θ ⊣⊢ₚ (persist P θ ->ₚ persist Q θ).
       Proof. obligation. Qed.
       Lemma persist_wand {w0 w1} (θ : Θ w0 w1) (P Q : Pred w0) :
-        persist (wandₚ P Q) θ ⊣⊢ₚ wandₚ (persist P θ) (persist Q θ).
-      Proof. now rewrite ?wand_is_impl persist_impl. Qed.
+        persist (interface.bi_wand P Q) θ ⊣⊢ₚ interface.bi_wand (persist P θ) (persist Q θ).
+      Proof. obligation. Qed.
       Lemma persist_false {w0 w1} (θ : Θ w0 w1) :
         persist ⊥ₚ θ ⊣⊢ₚ ⊥ₚ.
       Proof. obligation. Qed.
       Lemma persist_true {w0 w1} (θ : Θ w0 w1) :
         persist ⊤ₚ θ ⊣⊢ₚ ⊤ₚ.
       Proof. obligation. Qed.
-      Lemma persist_eq {T : TYPE} {persR : Persistence.Persistent T}
-        {A : Type} {instTA : Inst T A} {instPersistTA : InstPersist T A}
-        {w0 w1} (θ : Θ w0 w1) (t1 t2 : T w0) :
-        persist (t1 =ₚ t2) θ ⊣⊢ₚ persist t1 θ =ₚ persist t2 θ.
-      Proof.
-        constructor. unfold eqₚ, persist, persist_pred. intros ι.
-        now rewrite !inst_persist.
-      Qed.
-
       Lemma persist_forall [A] [w0 w1] (θ : Θ w0 w1) (Q : A -> Pred w0) :
         persist (∀ₚ a : A, Q a) θ ⊣⊢ₚ (∀ₚ a : A, persist (Q a) θ).
       Proof. obligation. Qed.
@@ -500,10 +468,9 @@ Module Pred.
   End Lemmas.
 
   Module Acc.
-    Import World.notations.
     Import (hints) Sub.
     Section WithAccessibilityRelation.
-      Context {Θ : ACC}.
+      Context {Θ : SUB}.
 
       Definition wp {w0 w1} (θ : Θ w0 w1) (Q : Pred w1) : Pred w0 :=
         fun ι0 => exists (ι1 : Assignment w1), inst θ ι1 = ι0 /\ Q ι1.
@@ -518,7 +485,7 @@ Module Pred.
       Proof. firstorder. Qed.
 
       #[export] Instance proper_wp_entails {w0 w1} (θ : Θ w0 w1) :
-        Proper (entails ==> entails) (wp θ).
+        Proper ((⊢ₚ) ==> (⊢ₚ)) (wp θ).
       Proof. firstorder. Qed.
 
       #[export] Instance proper_wlp_bientails {w0 w1} (θ : Θ w0 w1) :
@@ -526,26 +493,24 @@ Module Pred.
       Proof. firstorder. Qed.
 
       #[export] Instance proper_wlp_entails {w0 w1} (θ : Θ w0 w1) :
-        Proper (entails ==> entails) (wlp θ).
+        Proper ((⊢ₚ) ==> (⊢ₚ)) (wlp θ).
       Proof. firstorder. Qed.
 
       Lemma wp_refl {reflΘ : Refl Θ} {lkreflΘ : LkRefl Θ}
         {w} (Q : Pred w) : wp refl Q ⊣⊢ₚ Q.
       Proof.
-        constructor. split; cbn.
-        - intros (ι' & Heq & HQ). rewrite inst_refl in Heq. now subst.
-        - intros HQ. exists ι. split. now rewrite inst_refl. easy.
+        unfold wp; pred_unfold. intros ι; split.
+        - intros (ι' & Heq & HQ). now subst.
+        - intros HQ. exists ι. easy.
       Qed.
 
       Lemma wp_trans {transR : Trans Θ} {lktransΘ : LkTrans Θ}
         {w0 w1 w2} (θ1 : Θ w0 w1) (θ2 : Θ w1 w2) Q :
         wp (θ1 ⊙ θ2) Q ⊣⊢ₚ wp θ1 (wp θ2 Q).
       Proof.
-        constructor. split; cbn.
-        - intros (ι2 & Heq & HQ). rewrite inst_trans in Heq.
-          exists (inst θ2 ι2). split. easy. now exists ι2.
-        - intros (ι1 & Heq1 & ι2 & Heq2 & HQ). exists ι2.
-          split; [|easy]. rewrite inst_trans. congruence.
+        unfold wp; pred_unfold. intros ι; split.
+        - intros (ι2 & Heq & HQ). eauto.
+        - intros (ι1 & Heq1 & ι2 & Heq2 & HQ). subst. eauto.
       Qed.
 
       Lemma wp_false {w0 w1} (θ : Θ w0 w1) :
@@ -555,12 +520,12 @@ Module Pred.
       Lemma and_wp_l {w0 w1} (θ : Θ w0 w1) P Q :
         wp θ P /\ₚ Q ⊣⊢ₚ wp θ (P /\ₚ persist Q θ).
       Proof.
-        constructor. split; cbn.
-        - intros [(ι1 & <- & HP) HQ]. now exists ι1.
-        - intros (ι1 & <- & HP & HQ). split; [|easy]. now exists ι1.
+        unfold wp; pred_unfold. split.
+        - intros [(ι1 & <- & HP) HQ]. eauto.
+        - intros (ι1 & <- & HP & HQ). eauto.
       Qed.
 
-      Lemma and_wp_r {w0 w1} (θ : Θ w0 w1) P Q :
+      Lemma and_wp_r {w0 w1} (θ : Θ w0 w1) (P : Pred w0) (Q : Pred w1) :
         P /\ₚ wp θ Q ⊣⊢ₚ wp θ (persist P θ /\ₚ Q).
       Proof. now rewrite and_comm, and_wp_l, and_comm. Qed.
 
@@ -568,35 +533,32 @@ Module Pred.
         {w α} (αIn : world.In α w) (t : Ṫy (w - α)) (Q : Pred (w - α)) :
         wp (thick α t) Q ⊣⊢ₚ ṫy.var αIn =ₚ persist t (thin (Θ := Sub) α) /\ₚ persist Q (thin (Θ := Sub) α).
       Proof.
-        constructor. intros ι; pred_unfold; cbn. rewrite inst_thin.
-        split.
+        unfold wp; pred_unfold. intros ι. split.
         - intros (ι1 & Heq & HQ). subst.
           now rewrite inst_thick, env.remove_insert, env.lookup_insert.
         - intros [Heq HQ]. exists (env.remove α ι αIn).
-          rewrite inst_thick. rewrite <- Heq. now rewrite env.insert_remove.
+          now rewrite inst_thick, <- Heq, env.insert_remove.
       Qed.
 
       Lemma wlp_refl {reflΘ : Refl Θ} {lkreflΘ : LkRefl Θ}
         {w} (Q : Pred w) : wlp refl Q ⊣⊢ₚ Q.
       Proof.
-        constructor. split; cbn.
-        - intros HQ. apply HQ. now rewrite inst_refl.
-        - intros HQ ? <-. now rewrite inst_refl in HQ.
+        unfold wlp; pred_unfold. intros ι. split.
+        - intros HQ. auto.
+        - intros HQ ? <-. auto.
       Qed.
 
       Lemma wlp_trans {transR : Trans Θ} {lktransΘ : LkTrans Θ}
         {w0 w1 w2} (θ1 : Θ w0 w1) (θ2 : Θ w1 w2) Q :
         wlp (θ1 ⊙ θ2) Q ⊣⊢ₚ wlp θ1 (wlp θ2 Q).
       Proof.
-        constructor. split; cbn.
-        - intros HQ ι1 Heq1 ι2 Heq2. apply HQ.
-          subst. now rewrite inst_trans.
-        - intros HQ ι2 Heq. rewrite inst_trans in Heq.
-          now apply (HQ (inst θ2 ι2)).
+        unfold wlp; pred_unfold. intros ι. split.
+        - intros HQ ι1 Heq1 ι2 Heq2. subst; auto.
+        - intros HQ ι2 Heq. subst; eauto.
       Qed.
 
       Lemma wlp_true {w0 w1} (θ : Θ w0 w1) :
-        wlp θ Trueₚ ⊣⊢ₚ Trueₚ.
+        wlp θ ⊤ₚ ⊣⊢ₚ ⊤ₚ.
       Proof. firstorder. Qed.
 
       Lemma wlp_and {w0 w1} (θ : Θ w0 w1) P Q :
@@ -608,17 +570,17 @@ Module Pred.
       Proof. firstorder. Qed.
 
       Lemma wp_mono {w0 w1} (θ : Θ w0 w1) P Q:
-        wlp θ (P ->ₚ Q) ⊢ₚ (wp θ P ->ₚ wp θ Q).
+        wlp θ (interface.bi_wand P Q) ⊢ₚ interface.bi_wand (wp θ P) (wp θ Q).
       Proof. firstorder. Qed.
 
       Lemma wlp_mono {w0 w1} (θ : Θ w0 w1) P Q :
-        wlp θ (P ->ₚ Q) ⊢ₚ wlp θ P ->ₚ wlp θ Q.
+        wlp θ (interface.bi_wand P Q) ⊢ₚ interface.bi_wand (wlp θ P) (wlp θ Q).
       Proof. firstorder. Qed.
 
       Lemma entails_wlp {w0 w1} (θ : Θ w0 w1) P Q :
         (persist P θ ⊢ₚ Q) <-> (P ⊢ₚ wlp θ Q).
       Proof.
-        split; intros [HPQ]; constructor.
+        unfold wlp; pred_unfold. split; intros HPQ.
         - intros ι0 HP ι1 <-. revert HP. apply HPQ.
         - intros ι1 HP. now apply (HPQ (inst θ ι1)).
       Qed.
@@ -626,7 +588,7 @@ Module Pred.
       Lemma entails_wp {w0 w1} (θ : Θ w0 w1) P Q :
         (P ⊢ₚ persist Q θ) <-> (wp θ P ⊢ₚ Q).
       Proof.
-        split; intros [HPQ]; constructor.
+        unfold wp; pred_unfold. split; intros HPQ.
         - intros ι0 (ι1 & <- & HP). now apply HPQ.
         - intros ι1 HP. apply (HPQ (inst θ ι1)).
           exists ι1. split; auto.
@@ -635,8 +597,7 @@ Module Pred.
       Lemma wp_impl {w0 w1} (θ1 : Θ w0 w1) (P : Pred _) (Q : Pred _) :
         (wp θ1 P ->ₚ Q) ⊣⊢ₚ wlp θ1 (P ->ₚ persist Q θ1).
       Proof.
-        constructor. intros ι; unfold wp, wlp. pred_unfold.
-        split.
+        unfold wp, wlp; pred_unfold. intros ι0; split.
         - intros H ι1 <- HP. apply H. now exists ι1.
         - intros HPQ (ι1 & <- & HP). now apply HPQ.
       Qed.
@@ -652,8 +613,7 @@ Module Pred.
       Lemma wlp_frame {w0 w1} (θ : Θ w0 w1) (P : Pred _) (Q : Pred _) :
         P ->ₚ wlp θ Q ⊣⊢ₚ wlp θ (persist P θ ->ₚ Q).
       Proof.
-        constructor. intros ι.
-        split; cbv [wlp interface.bi_impl bi_pred implₚ].
+        unfold wlp; pred_unfold. intros ι; split.
         - intros H ι1 <- HP. now apply (H HP).
         - intros H HP ι1 <-. apply H; auto.
       Qed.
@@ -662,173 +622,103 @@ Module Pred.
     (* #[global] Opaque wp. *)
     (* #[global] Opaque wlp. *)
 
-    Lemma proper_wp_step {Θ1 Θ2 : ACC} {stepΘ1 : Step Θ1} {stepΘ2 : Step Θ2}
-      {lkStepΘ1 : LkStep Θ1} {lkStepΘ2 : LkStep Θ2}
-      {w α} :
-      forall P Q : Pred (world.snoc w α),
-        P ⊣⊢ₚ Q -> wp (step (Θ := Θ1)) P ⊣⊢ₚ wp (step (Θ := Θ2)) Q.
+    (* Lemma proper_wp_step {Θ1 Θ2 : SUB} {stepΘ1 : Step Θ1} {stepΘ2 : Step Θ2} *)
+    (*   {lkStepΘ1 : LkStep Θ1} {lkStepΘ2 : LkStep Θ2} *)
+    (*   {w α} : *)
+    (*   forall P Q : Pred (world.snoc w α), *)
+    (*     P ⊣⊢ₚ Q -> wp (step (Θ := Θ1)) P ⊣⊢ₚ wp (step (Θ := Θ2)) Q. *)
+    (* Proof. *)
+    (*   intros P Q [PQ]. constructor. intros ι. apply base.exist_proper. *)
+    (*   intros ι2. now rewrite !inst_step, PQ. *)
+    (* Qed. *)
+
+    Lemma intro_wp_step' {Θ} {stepΘ : Step Θ} {lkStepΘ : LkStep Θ}
+      {w α} (P : Pred w) (Q : Pred (world.snoc w α)) (t : Ty) :
+      (persist P step ⊢ₚ lift t =ₚ @ṫy.var _ α world.in_zero ->ₚ Q) ->
+      (P ⊢ₚ wp (step (Θ := Θ)) Q).
     Proof.
-      intros P Q [PQ]. constructor. intros ι. cbn. apply base.exist_proper.
-      intros ι2. now rewrite !inst_step, PQ.
+      pred_unfold. intros H ι HP. set (ι1 := env.snoc ι α t).
+      exists ι1. specialize (H ι1). rewrite inst_step in *; cbn in *.
+      intuition.
     Qed.
 
+    (* Better for iris proof mode. *)
     Lemma intro_wp_step {Θ} {stepΘ : Step Θ} {lkStepΘ : LkStep Θ}
-      {w α} (Q : Pred (world.snoc w α)) :
-      wp (step (Θ := Θ)) Q ⊣⊢ₚ
-      ∃ₚ t : Ṫy _, wlp step (persist t step =ₚ ṫy.var world.in_zero ->ₚ Q).
+      t {w α} (Q : Pred (world.snoc w α)) :
+      wlp step (lift t =ₚ ṫy.var world.in_zero ->ₚ Q) ⊢ₚ wp (step (Θ := Θ)) Q.
+    Proof. apply (intro_wp_step' t). now rewrite persist_wlp. Qed.
+
+    Lemma wp_split  {Θ : SUB} [w0 w1] (θ : Θ w0 w1) P :
+      wp θ ⊤ₚ /\ₚ wlp θ P ⊢ₚ wp θ P.
+    Proof. now rewrite and_wp_l, persist_wlp, and_true_l. Qed.
+
+    Lemma wp_sub_of {Θ : SUB} [w0 w1] (θ : Θ w0 w1) P :
+      wp (Sub.of θ) P ⊣⊢ₚ wp θ P.
     Proof.
-      constructor. intros ι. pred_unfold. unfold wlp, wp, implₚ, eqₚ. cbn.
-      split.
-      - intros (ι' & Heq & HQ). subst. destruct (env.view ι').
-        exists (lift v). intros ι' Heq1 Heq2.
-        rewrite inst_step_snoc in Heq1. subst.
-        rewrite inst_persist, inst_lift in Heq2. subst.
-        destruct (env.view ι'). rewrite inst_step_snoc in HQ.
-        now cbn in HQ.
-      - intros (t & H). exists (env.snoc ι α (inst t ι)).
-        rewrite inst_step_snoc. split; [easy|]. apply H.
-        + now rewrite inst_step_snoc.
-        + now rewrite inst_persist, inst_step_snoc.
+      constructor. intros ι0; cbn. apply ex_iff_morphism; intro ι1.
+      apply and_iff_compat_r.
+      split; intros; subst; apply env.lookup_extensional; intros α αIn;
+        unfold Sub.of, inst, inst_acc, lk; cbn; now rewrite !env.lookup_tabulate.
+    Qed.
+
+    Lemma wlp_sub_of {Θ : SUB} [w0 w1] (θ : Θ w0 w1) P :
+      wlp (Sub.of θ) P ⊣⊢ₚ wlp θ P.
+    Proof.
+      constructor. intros ι0; cbn. apply all_iff_morphism; intro ι1.
+      apply imp_iff_compat_r.
+      split; intros; subst; apply env.lookup_extensional; intros α αIn;
+        unfold Sub.of, inst, inst_acc, lk; cbn; now rewrite !env.lookup_tabulate.
     Qed.
 
   End Acc.
 
-  Section Transformers.
-    Import World.notations.
-    Import (hints) Diamond.
-
-    Definition wp_diamond {Θ : ACC} {A} :
-      ⊧ Diamond Θ A ⇢ Box Θ (A ⇢ Pred) ⇢ Pred :=
-      fun w '(existT w1 (θ, a)) Q => Acc.wp θ (Q w1 θ a).
-
-    Definition wp_option {A w1 w2} :
-      Option A w1 -> (A w1 -> Pred w2) -> Pred w2 :=
-      fun o Q =>
-        match o with
-        | Some a => Q a
-        | None => Falseₚ
-        end.
-
-    Lemma wp_option_bind {A B w1 w2 w3} (o : Option A w1)
-      (f : A w1 -> Option B w2) (Q : B w2 -> Pred w3) :
-      wp_option (option.bind o f) Q ⊣⊢ₚ wp_option o (fun a => wp_option (f a) Q).
-    Proof. constructor; intros ι. now destruct o. Qed.
-
-    Lemma wp_option_map {A B : TYPE} {w1 w2 w3} (o : Option A w1)
-      (f : A w1 -> B w2) (Q : B w2 -> Pred w3) :
-      wp_option (option.map f o) Q ⊣⊢ₚ wp_option o (fun a => Q (f a)).
-    Proof. constructor; intros ι. now destruct o. Qed.
-
-    Definition wp_optiondiamond {Θ : ACC} {A} :
-      ⊧ DiamondT Θ Option A ⇢ Box Θ (A ⇢ Pred) ⇢ Pred :=
-      fun w m Q => wp_option m (fun d => wp_diamond d Q).
-
-    #[global] Arguments wp_optiondiamond {Θ} {A}%indexed_scope [w] _ _%B _.
-    #[global] Instance params_wp_optiondiamond : Params (@wp_optiondiamond) 5 := {}.
-
-    #[export] Instance proper_wp_optiondiamond_bientails {Θ A w} :
-      Proper
-        (pointwise_relation _
-           (forall_relation
-              (fun _ => pointwise_relation _
-                          (pointwise_relation _ bientails)) ==> bientails))
-        (@wp_optiondiamond Θ A w).
-    Proof.
-      intros d p q pq. destruct d as [(w1 & r01 & a)|]; cbn; [|easy].
-      apply Acc.proper_wp_bientails. apply pq.
-    Qed.
-
-    #[export] Instance proper_wp_optiondiamond_entails {Θ A w} :
-      Proper
-        (pointwise_relation _
-           (forall_relation
-              (fun _ => pointwise_relation _
-                          (pointwise_relation _ entails)) ==> entails))
-        (@wp_optiondiamond Θ A w).
-    Proof.
-      intros d p q pq. destruct d as [(w1 & r01 & a)|]; cbn; [|easy].
-      apply Acc.proper_wp_entails. apply pq.
-    Qed.
-
-    Lemma wp_optiondiamond_and {Θ A w} (d : DiamondT Θ Option A w)
-      (P : Box Θ (A ⇢ Pred) w) (Q : Pred w) :
-       wp_optiondiamond d P /\ₚ Q
-       ⊣⊢ₚ wp_optiondiamond d (fun w1 θ1 a1 => P w1 θ1 a1 /\ₚ persist Q θ1).
-    Proof.
-      destruct d as [(w1 & θ1 & a1)|]; cbn.
-      - now rewrite Acc.and_wp_l.
-      - now rewrite and_false_l.
-    Qed.
-
-    Lemma wp_optiondiamond_monotonic' {Θ A w} (d : DiamondT Θ Option A w)
-      (R : Pred w) (P Q : Box Θ (A ⇢ Pred) w) :
-      (forall w1 (r : Θ w w1) (a : A w1),
-          persist R r ⊢ₚ P w1 r a ->ₚ Q w1 r a) ->
-      R ⊢ₚ wp_optiondiamond d P ->ₚ wp_optiondiamond d Q.
-    Proof.
-      intros pq. destruct d as [(w1 & r01 & a)|]; cbn.
-      - specialize (pq w1 r01 a).
-        apply impl_and_adjoint.
-        rewrite Acc.and_wp_r.
-        apply Acc.proper_wp_entails.
-        apply impl_and_adjoint.
-        apply pq.
-      - apply impl_and_adjoint.
-        now rewrite and_false_r.
-    Qed.
-
-    Lemma wp_optiondiamond_pure {Θ} {reflΘ : Refl Θ} {lkreflΘ : LkRefl Θ}
-      {A w0} (a : A w0) (Q : Box Θ (A ⇢ Pred) w0) :
-      wp_optiondiamond (pure (M := DiamondT Θ Option) a) Q ⊣⊢ₚ T Q a.
-    Proof. cbn. now rewrite Acc.wp_refl. Qed.
-
-    Lemma wp_optiondiamond_bind {Θ} {transΘ : Trans Θ} {lkTransΘ : LkTrans Θ}
-      {A B w0} (d : DiamondT Θ Option A w0) (f : Box Θ (A ⇢ DiamondT Θ Option B) w0)
-      (Q : Box Θ (B  ⇢ Pred) w0) :
-      wp_optiondiamond (bind d f) Q ⊣⊢ₚ
-      wp_optiondiamond d (fun w1 ζ1 a1 => wp_optiondiamond (f w1 ζ1 a1) Q[ζ1]).
-    Proof.
-      destruct d as [(w1 & r01 & a)|]; cbn; [|reflexivity].
-      destruct (f w1 r01 a) as [(w2 & r12 & b2)|]; cbn;
-        now rewrite ?Acc.wp_trans, ?Acc.wp_false.
-    Qed.
-
-    Lemma wp_optiondiamond_bind' {Θ : ACC} {A B w1 w2} (o : Option A w1)
-      (f : A w1 -> Option (Diamond Θ B) w2) (Q : Box Θ (B ⇢ Pred) w2) :
-      wp_optiondiamond (option.bind o f) Q ⊣⊢ₚ
-      wp_option o (fun a => wp_optiondiamond (f a) Q).
-    Proof. constructor; intros ι. now destruct o. Qed.
-
-  End Transformers.
-
   Section InstPred.
-    Import World.notations.
+    Import iris.bi.derived_laws.
+    Import iris.bi.interface.
+    Import Stlc.Persistence.
     (* A type class for things that can be interpreted as a predicate. *)
     Class InstPred (A : TYPE) :=
       instpred : ⊧ A ⇢ Pred.
     #[global] Arguments instpred {_ _ _}.
 
-    #[export] Instance instpred_option {A} `{ipA : InstPred A} :
-      InstPred (Option A) :=
-      fun w o => wp_option o instpred.
+    (* #[export] Instance instpred_option {A} `{ipA : InstPred A} : *)
+    (*   InstPred (Option A) := *)
+    (*   fun w o => wp_option o instpred. *)
     #[export] Instance instpred_list {A} `{ipA : InstPred A} :
       InstPred (List A) :=
       fun w =>
         fix ip xs {struct xs} :=
         match xs with
-        | nil       => Trueₚ
-        | cons y ys => andₚ (instpred y) (ip ys)
-        end.
+        | nil       => ⊤ₚ
+        | cons y ys => instpred y /\ₚ ip ys
+        end%P.
     #[local] Instance instpred_prod_ty : InstPred (Ṫy * Ṫy) :=
       fun w '(t1,t2) => eqₚ t1 t2.
     #[export] Instance instpred_unit : InstPred Unit :=
-      fun w 'tt => Trueₚ.
-    #[local] Instance instpred_diamond {Θ A} `{ipA : InstPred A} :
-      InstPred (Diamond Θ A) :=
-      fun w m => wp_diamond m (fun _ _ a => instpred a).
-    #[export] Instance instpred_optiondiamond {Θ A} `{ipA : InstPred A} :
-      InstPred (DiamondT Θ Option A) :=
-      fun w m => wp_optiondiamond m (fun _ _ a => instpred a).
+      fun w 'tt => ⊤ₚ%P.
+
+    Lemma instpred_list_app {A} `{ipA : InstPred A} [w] (xs ys : List A w) :
+      instpred (xs ++ ys) ⊣⊢ₚ instpred xs /\ₚ instpred ys.
+    Proof.
+      induction xs; cbn.
+      - now rewrite and_true_l.
+      - rewrite Pred.and_assoc. now apply bi.and_proper.
+    Qed.
+
+    Class InstPredPersist A {ipA : InstPred A} {persA : Persistent A} :=
+      instpred_persist [Θ : SUB] {w0 w1} (θ : Θ w0 w1) (a : A w0) :
+        instpred (persist a θ) ⊣⊢ₚ persist (instpred a) θ.
+    #[global] Arguments InstPredPersist _ {_ _}.
+
+    #[export] Instance instpred_persist_list `{InstPredPersist A} :
+      InstPredPersist (List A).
+    Proof.
+      intros Θ w0 w1 θ xs. unfold persist, persistent_list.
+      induction xs; cbn; [easy|]. now rewrite instpred_persist IHxs.
+    Qed.
+
+    #[local] Instance instpred_persist_prod_ty : InstPredPersist (Ṫy * Ṫy).
+    Proof. intros Θ w0 w1 θ [τ1 τ2]; cbn. now rewrite persist_eq. Qed.
 
   End InstPred.
 
@@ -841,23 +731,23 @@ Module Pred.
 
   Lemma eqₚ_insert {w} (G1 G2 : Ėnv w) (x : string) (t1 t2 : Ṫy w) :
     G1 =ₚ G2 /\ₚ t1 =ₚ t2 ⊢ₚ
-    (G1 ,, x ∷ t1) =ₚ (G2 ,, x ∷ t2).
-  Proof. constructor. intros ι []. now pred_unfold. Qed.
+    insert (M := Ėnv w) x t1 G1 =ₚ insert (M := Ėnv w) x t2 G2.
+  Proof. pred_unfold. intros []. now f_equal. Qed.
 
   Lemma eq_func {w} (s1 s2 t1 t2 : Ṫy w) :
     ṫy.func s1 s2 =ₚ ṫy.func t1 t2 ⊣⊢ₚ (s1 =ₚ t1) /\ₚ (s2 =ₚ t2).
   Proof. now rewrite peq_ty_noconfusion. Qed.
 
-  #[export] Instance params_tpb : Params (@TPB) 5 := {}.
-  #[export] Instance params_ifte : Params (@ėxp.ifte) 4 := {}.
-  #[export] Instance params_eqₚ : Params (@eqₚ) 6 := {}.
-  #[export] Instance params_persist : Params (@persist) 7 := {}.
+  #[export] Instance params_tpb : Params (@TPB) 1 := {}.
+  #[export] Instance params_ifte : Params (@ėxp.ifte) 1 := {}.
+  #[export] Instance params_eqₚ : Params (@eqₚ) 4 := {}.
+  #[export] Instance params_persist : Params (@persist) 4 := {}.
 
   Section AccModality.
 
     Import iris.proofmode.tactics.
 
-    Context {Θ : ACC} [w0 w1] (θ : Θ w0 w1).
+    Context {Θ : SUB} [w0 w1] (θ : Θ w0 w1).
 
     Class IntoAcc (P : Pred w0) (Q : Pred w1) :=
       into_acc : P ⊢ Acc.wlp θ Q.
@@ -884,19 +774,73 @@ Module Pred.
   #[global] Arguments into_acc {Θ} [w0 w1] θ P Q {_}.
   #[global] Hint Mode IntoAcc + + + + - - : typeclass_instances.
 
-  Create HintDb predsimpl.
+  Import (hints) Sub.
 
-  #[export] Hint Rewrite (@persist_refl Ėnv _ _) (@persist_refl Ṫy _ _)
-    (@persist_trans Ėnv _ _) (@persist_trans Ṫy _ _) @persist_eq @persist_tpb
-    @persist_and @persist_insert @persist_lift @lift_insert @Sem.persist_pure
-    @impl_and @and_false_l @impl_true_l @eqₚ_refl @eq_func @and_true_l
-    @Acc.wp_false @lk_trans : predsimpl.
+  Create HintDb predsimpl.
+  #[export] Hint Rewrite
+    (@persist_eq Ėnv _ _ _ _)
+    (@persist_eq Ṫy _ _ _ _)
+    (@persist_refl Ėnv _ _)
+    (@persist_refl Ṫy _ _)
+    (@persist_trans Ėnv _ _)
+    (@persist_trans Ṫy _ _)
+    @Acc.wlp_refl
+    @Acc.wlp_trans
+    @Acc.wlp_true
+    @Acc.wp_false
+    @Acc.wp_refl
+    @Acc.wp_trans
+    @Sem.persist_pure
+    @and_false_l
+    @and_false_r
+    @and_true_l
+    @and_true_r
+    @eq_func
+    @eqₚ_refl
+    @impl_and
+    @impl_false_l
+    @impl_true_l
+    @impl_true_r
+    @lift_insert
+    @lk_refl
+    @lk_step
+    @lk_trans
+    @persist_and
+    @persist_false
+    @persist_insert
+    @persist_lift
+    @persist_pred_refl
+    @persist_pred_trans
+    @persist_tpb
+    @persist_true
+    @trans_refl_r
+    : predsimpl.
   #[export] Hint Rewrite <- @eqₚ_insert : predsimpl.
 
   Ltac predsimpl :=
     repeat
-      (try (progress cbn);
-       autorewrite with predsimpl; eauto with typeclass_instances;
+      (try (progress cbn); unfold _4;
+       change_no_check (@gmap.gmap string _ _ (Ṫy ?w)) with (Ėnv w) in *;
+       repeat
+         match goal with
+         | |- context[fun w : World => Ṫy w] =>
+             change_no_check (fun w : World => Ṫy w) with Ṫy
+         | |- context[fun w : World => Sem ?X w] =>
+             change_no_check (fun w : World => Sem X w) with (Sem X)
+         | |- context[fun w : World => prod (?A w) (?B w)] =>
+             change_no_check (fun w : World => prod (A w) (B w)) with (Prod A B)
+
+         | |- Acc.wp ?θ _ ⊣⊢ₚ Acc.wp ?θ _ =>
+             apply Acc.proper_wp_bientails
+         | |- Acc.wlp ?θ _ ⊣⊢ₚ Acc.wlp ?θ _ =>
+             apply Acc.proper_wlp_bientails
+         end;
+       try easy;
+       repeat rewrite_db predsimpl;
+       repeat rewrite ?trans_refl_r, ?persist_eq, ?persist_lift,
+         ?persist_pred_refl, ?persist_tpb, ?persist_trans, ?persist_trans,
+         <- ?persist_pred_trans;
+       auto 1 with typeclass_instances;
        repeat
          match goal with
          | |- context[@persist ?A ?I ?Θ ?w0 ?x ?w1 ?θ] =>
@@ -906,10 +850,6 @@ Module Pred.
              is_var θ;
              generalize (@lk Θ (world.snoc w0 α) w1 θ α world.in_zero);
              clear θ w0; intros ?t
-         | |- context[fun w : World => Ṫy w] =>
-             change_no_check (fun w : World => Ṫy w) with Ṫy
-         | |- context[fun w : World => Sem ?X w] =>
-             change_no_check (fun w : World => Sem X w) with (Sem X)
          end).
 
 End Pred.
