theories/Stlc/PrenexConversion.v
@@ -26,76 +26,54 @@
 (* SOFTWARE, EVEN IF ADVISED OF THE POSSIBILITY OF SUCH DAMAGE.               *)
 (******************************************************************************)
 
+From Coq Require Import
+  Strings.String.
+From Equations Require Import
+  Equations.
 From Em Require Import
   Prelude
+  Stlc.Alloc
+  Stlc.MonadInterface
+  Stlc.MonadFree
+  Stlc.MonadPrenex
+  Stlc.Instantiation
   Stlc.Persistence
+  Stlc.Predicates
   Stlc.Spec
+  Stlc.Substitution
   Stlc.Worlds.
 
 Import world.notations.
+Import option.notations.
+Import Pred Pred.notations.
+Import (hints) Pred.Acc.
 
 #[local] Set Implicit Arguments.
 
-Module alloc.
-
-  Inductive Rel (w : World) : TYPE :=
-  | refl        : Rel w w
-  | snoc {w' α} : Rel w w' → Rel w (w' ▻ α).
-  #[global] Arguments refl {_}.
-  #[global] Arguments snoc {_ _ _} _.
-
-  Fixpoint persist_in {w0 w1} (θ : Rel w0 w1) [α] (αIn : α ∈ w0) : α ∈ w1 :=
-    match θ with
-    | refl    => αIn
-    | snoc θ' => world.in_succ (persist_in θ' αIn)
+Definition prenex {A} : ⊧ Free A ⇢ Prenex A :=
+  fix pr {w} m {struct m} :=
+    match m with
+    | Ret a => pure a
+    | Fail => None
+    | Assertk t1 t2 m =>
+        '(existT w1 (r1, (cs, a))) <- pr m;;
+        let t1' := persist t1 r1 in
+        let t2' := persist t2 r1 in
+        let c   := (t1', t2') in
+        Some (existT w1 (r1, (cons c cs, a)))
+    | Choosek α m =>
+        '(existT w1 (r1, csa)) <- pr m ;;
+        Some (existT w1 (step ⊙ r1, csa))
     end.
 
-  Canonical Structure Alloc : SUB :=
-    {| sub              := Rel;
-       lk w0 w1 θ α αIn := ṫy.var (persist_in θ αIn)
-    |}.
-
-  #[export] Instance refl_alloc : Refl Alloc :=
-    fun w => refl.
-  #[export] Instance trans_alloc : Trans Alloc :=
-    fix trans {w0 w1 w2} (θ1 : Alloc w0 w1) (θ2 : Alloc w1 w2) : Alloc w0 w2 :=
-      match θ2 with
-      | refl     => θ1
-      | snoc θ2' => snoc (trans θ1 θ2')
-      end.
-
-  #[export] Instance step_alloc : Step Alloc :=
-    fun w α => snoc refl.
-  #[export] Instance refltrans_alloc : ReflTrans Alloc.
-  Proof.
-    constructor.
-    - intros ? ? θ; induction θ; cbn; now f_equal.
-    - easy.
-    - intros ? ? ? ? θ1 θ2 θ3. induction θ3; cbn; now f_equal.
-  Qed.
-
-  Fixpoint nil {w} : Alloc world.nil w :=
-    match w with
-    | ε      => refl
-    | w' ▻ α => snoc nil
-    end.
-
-  #[export] Instance lkrefl : LkRefl Alloc.
-  Proof. easy. Qed.
-  #[export] Instance lktrans : LkTrans Alloc.
-  Proof.
-    intros w0 w1 w2 θ1 θ2 α αIn. do 2 (unfold lk; cbn).
-    f_equal. induction θ2; cbn; now f_equal.
-  Qed.
-  #[export] Instance lkstep : LkStep Alloc.
-  Proof. easy. Qed.
-
-End alloc.
-Export alloc (Alloc).
-Export (hints) alloc.
-Notation "w1 ⊑⁺ w2" := (sub Alloc w1 w2) (at level 80).
-Infix "⊙⁺" := (trans (Θ := Alloc)) (at level 60, right associativity).
-Notation "□⁺ A" := (Box Alloc A)
-  (at level 9, right associativity, format "□⁺ A") : indexed_scope.
-Notation "◇⁺ A" := (Diamond Alloc A)
-  (at level 9, right associativity, format "◇⁺ A") : indexed_scope.
+Lemma prenex_correct {A w} (m : Free A w) (Q : Box Alloc (A ⇢ Pred) w) :
+  WP (prenex m) Q ⊣⊢ₚ WP m Q.
+Proof.
+  induction m; predsimpl.
+  - rewrite <- IHm. clear IHm.
+    destruct (prenex m) as [(w1 & θ1 & C1 & a1)|]; predsimpl.
+    rewrite Acc.and_wp_r. apply Acc.proper_wp_bientails. predsimpl.
+    now rewrite and_assoc.
+  - rewrite <- IHm. clear IHm.
+    destruct (prenex m) as [(w1 & θ1 & C1 & a1)|]; predsimpl.
+Qed.
