theories/Stlc/GeneratorSynthesise.v
@@ -1,0 +1,271 @@
+(******************************************************************************)
+(* Copyright (c) 2023 Denis Carnier, Steven Keuchel                           *)
+(* All rights reserved.                                                       *)
+(*                                                                            *)
+(* Redistribution and use in source and binary forms, with or without         *)
+(* modification, are permitted provided that the following conditions are     *)
+(* met:                                                                       *)
+(*                                                                            *)
+(* 1. Redistributions of source code must retain the above copyright notice,  *)
+(*    this list of conditions and the following disclaimer.                   *)
+(*                                                                            *)
+(* 2. Redistributions in binary form must reproduce the above copyright       *)
+(*    notice, this list of conditions and the following disclaimer in the     *)
+(*    documentation and/or other materials provided with the distribution.    *)
+(*                                                                            *)
+(* THIS SOFTWARE IS PROVIDED BY THE COPYRIGHT HOLDERS AND CONTRIBUTORS        *)
+(* "AS IS" AND ANY EXPRESS OR IMPLIED WARRANTIES, INCLUDING, BUT NOT LIMITED  *)
+(* TO, THE IMPLIED WARRANTIES OF MERCHANTABILITY AND FITNESS FOR A PARTICULAR *)
+(* PURPOSE ARE DISCLAIMED. IN NO EVENT SHALL THE COPYRIGHT HOLDER OR          *)
+(* CONTRIBUTORS BE LIABLE FOR ANY DIRECT, INDIRECT, INCIDENTAL, SPECIAL,      *)
+(* EXEMPLARY, OR CONSEQUENTIAL DAMAGES (INCLUDING, BUT NOT LIMITED TO,        *)
+(* PROCUREMENT OF SUBSTITUTE GOODS OR SERVICES; LOSS OF USE, DATA, OR         *)
+(* PROFITS; OR BUSINESS INTERRUPTION) HOWEVER CAUSED AND ON ANY THEORY OF     *)
+(* LIABILITY, WHETHER IN CONTRACT, STRICT LIABILITY, OR TORT (INCLUDING       *)
+(* NEGLIGENCE OR OTHERWISE) ARISING IN ANY WAY OUT OF THE USE OF THIS         *)
+(* SOFTWARE, EVEN IF ADVISED OF THE POSSIBILITY OF SUCH DAMAGE.               *)
+(******************************************************************************)
+
+From Coq Require Import
+  Strings.String.
+From Equations Require Import
+  Equations.
+From stdpp Require Import
+  base gmap.
+From iris Require Import
+  proofmode.tactics.
+From Em Require Import
+  Environment
+  Prelude
+  Stlc.Alloc
+  Stlc.Instantiation
+  Stlc.MonadInterface
+  Stlc.Persistence
+  Stlc.Predicates
+  Stlc.Sem
+  Stlc.Spec
+  Stlc.Worlds.
+
+Import world.notations.
+Import Pred Pred.notations.
+Import Pred.proofmode.
+
+Set Implicit Arguments.
+
+#[local] Notation "s [ ζ ]" :=
+  (persist s ζ)
+    (at level 7, left associativity,
+      format "s [ ζ ]").
+
+Section Generator.
+  Import MonadNotations.
+
+
+  Context {Θ} {reflΘ : Refl Θ} {stepΘ : Step Θ} {transΘ : Trans Θ}
+    {reflTransΘ : ReflTrans Θ} {lkReflΘ : LkRefl Θ} {lkTransΘ : LkTrans Θ}
+    {lkStepΘ : LkStep Θ}.
+  Context {M} {pureM : Pure M} {bindM : Bind Θ M} {tcM : TypeCheckM M} .
+
+  Definition generate : Exp -> ⊧ Ėnv ⇢ M (Ṫy * Ėxp) :=
+    fix gen e {w} Γ :=
+      match e with
+      | exp.var x =>
+          match lookup x Γ with
+          | Some t => pure (t , ėxp.var x)
+          | None   => fail
+          end
+      | exp.true  => pure (ṫy.bool, ėxp.true)
+      | exp.false => pure (ṫy.bool, ėxp.false)
+      | exp.ifte e1 e2 e3 =>
+          '(t1,e1') <- gen e1 Γ ;;
+          '(t2,e2') <- gen e2 Γ[_] ;;
+          '(t3,e3') <- gen e3 Γ[_] ;;
+          _         <- assert ṫy.bool t1[_] ;;
+          _         <- assert t2[_] t3[_] ;;
+          pure (t3[_], ėxp.ifte e1'[_] e2'[_] e3'[_])
+      | exp.absu x e =>
+          t1       <- pick ;;
+          '(t2,e') <- gen e (insert (M := Ėnv _) x t1 Γ[_]) ;;
+          pure (ṫy.func t1[_] t2, ėxp.abst x t1[_] e')
+      | exp.abst x t1 e =>
+          '(t2,e') <- gen e (insert (M := Ėnv _) x (lift t1) Γ) ;;
+          pure (ṫy.func (lift t1) t2, ėxp.abst x (lift t1) e')
+      | exp.app e1 e2 =>
+          '(tf, e1') <- gen e1 Γ ;;
+          '(t1, e2') <- gen e2 Γ[_] ;;
+          t2 <- pick ;;
+          _  <- assert tf[_] (ṫy.func t1[_] t2) ;;
+          pure (t2[_], ėxp.app e1'[_] e2'[_])
+      end.
+
+  Import Pred Pred.notations.
+  Import Pred.proofmode.
+  Import iris.proofmode.tactics.
+  Open Scope pred_scope.
+
+  Context {wpM : WeakestPre Θ M} {wlpM : WeakestLiberalPre Θ M}
+    {tcLogicM : TypeCheckLogicM Θ M}.
+
+  Definition TPB_algo : ⊧ Ėnv ⇢ Const Exp ⇢ Ṫy ⇢ Ėxp ⇢ Pred :=
+    fun w0 G0 e t0 e0 =>
+    WP (generate e G0)
+      (fun w1 (θ1 : Θ w0 w1) '(t1,e1) =>
+         t0[θ1] =ₚ t1 /\ₚ e0[θ1] =ₚ e1).
+
+  Lemma generate_sound_aux e :
+    forall (w : World) (G : Ėnv w),
+      ⊢ WLP (generate e G) (fun w1 θ '(t,ee) => G[θ] |--ₚ e; t ~> ee).
+  Proof.
+    induction e; cbn; intros w G; unfold _4; predsimpl.
+    - destruct lookup eqn:?; predsimpl.
+      + rewrite wlp_pure. pred_unfold. constructor.
+        now rewrite lookup_inst Heqo.
+      + rewrite wlp_fail. easy.
+    - rewrite wlp_pure. pred_unfold. constructor.
+    - rewrite wlp_pure. pred_unfold. constructor.
+    - rewrite wlp_bind. iApply (wlp_mono' $! (IHe1 _ G)).
+      iIntros (w1 θ1 (t1 & e1')) "!> #HT1".
+      rewrite wlp_bind. iApply (wlp_mono' $! (IHe2 _ G[_])).
+      iIntros (w2 θ2 (t2 & e2')) "!> #HT2".
+      rewrite wlp_bind. iApply (wlp_mono' $! (IHe3 _ G[_])).
+      iIntros (w3 θ3 (t3 & e3')) "!> #HT3".
+      clear IHe1 IHe2 IHe3.
+
+      do 2 rewrite wlp_bind wlp_assert. rewrite wlp_pure.
+      iIntros "#Heq1 #Heq2". predsimpl.
+      iStopProof. pred_unfold. intros (HT1 & HT2 & HT3 & Heq1 & Heq2).
+      subst; now constructor.
+
+    - rewrite wlp_bind wlp_pick. iIntros "!>".
+      rewrite wlp_bind. set (α := world.fresh w).
+      iApply (wlp_mono' $! (IHe (w ▻ α) (G[step] ,, x∷ṫy.var world.in_zero))).
+      iIntros (w1 θ1 (t1 & e1')) "!> #HT".
+      rewrite wlp_pure. predsimpl.
+      generalize (lk θ1 world.in_zero). intros ?τ.
+      iStopProof. pred_unfold. now constructor.
+
+    - rewrite wlp_bind. iApply (wlp_mono' $! (IHe _ (G ,, x∷lift t))).
+      iIntros (w1 θ1 (t1 & e1')) "!> #HT".
+      rewrite wlp_pure. predsimpl.
+      iStopProof. pred_unfold. now constructor.
+    - rewrite wlp_bind. iApply (wlp_mono' $! (IHe1 _ G)).
+      iIntros (w1 θ1 (t1 & e1')) "!> #HT1".
+      rewrite wlp_bind. iApply (wlp_mono' $! (IHe2 _ G[_])).
+      iIntros (w2 θ2 (t11 & e2')) "!> #HT2".
+      clear IHe1 IHe2.
+      rewrite wlp_bind wlp_pick. iIntros "!>".
+      rewrite wlp_bind wlp_assert. iIntros "#Heq1".
+      rewrite wlp_pure. predsimpl.
+      generalize (@ṫy.var (w2 ▻ world.fresh w2) (world.fresh w2)
+                (@world.in_zero (world.fresh w2) w2)).
+      intros τ12.
+      iStopProof. pred_unfold. intros (HT1 & HT2 & Heq). subst.
+      econstructor; eauto.
+  Qed.
+
+  Lemma generate_sound (e : Exp) (w0 : World) (G0 : Ėnv w0) t0 e0 :
+    TPB_algo G0 e t0 e0 ⊢ₚ G0 |--ₚ e; t0 ~> e0.
+  Proof.
+    iStartProof. rewrite wand_is_impl. rewrite wp_impl.
+    iApply (wlp_mono' $! (@generate_sound_aux e w0 G0)).
+    iIntros (w1 θ1 [t e']) "!> HT". predsimpl.
+    iStopProof. pred_unfold. intros HT Heq1 Heq2. now subst.
+  Qed.
+
+  Lemma generate_complete_aux {G e t ee} (T : G |-- e ∷ t ~> ee) :
+    forall w0 (G0 : Ėnv w0),
+      ⊢ lift G =ₚ G0 →
+      WP (generate e G0)
+          (fun w1 θ1 '(t',e') => lift t =ₚ t' /\ₚ Sem.pure ee =ₚ e')%P.
+  Proof.
+    induction T as [G x t Hres|G|G|G e1 e1' e2 e2' e3 e3' t _ IH1 _ IH2 _ IH3
+      |G x t1 t2 e e' _ IH|G x t1 t2 e e' _ IH|G e1 t2 e1' e2 t1 e2' _ IH1 _ IH2];
+      intros w0 G0; predsimpl; unfold _4.
+
+    - pred_unfold. intros HEq. subst. rewrite lookup_inst in Hres.
+      apply noConfusion_inv in Hres.
+      destruct (G0 !! x); pred_unfold; cbn in Hres; [|easy].
+      subst. now apply wp_pure; pred_unfold.
+
+    - now rewrite wp_pure.
+    - now rewrite wp_pure.
+
+    - iIntros "#HeqG". rewrite wp_bind.
+      iPoseProof (IH1 _ G0 with "HeqG") as "-#IH".
+      iApply (wp_mono' with "IH").
+      iIntros (w1 r1 (t1 & e1'')) "!> (#Heq1 & #Heq2)".
+
+      predsimpl. rewrite wp_bind.
+      iPoseProof (IH2 _ G0[_] with "HeqG") as "-#IH".
+      iApply (wp_mono' with "IH").
+      iIntros (w2 r2 (t2 & e2'')) "!> (#Heq3 & #Heq4)".
+      predsimpl. rewrite wp_bind.
+      iPoseProof (IH3 _ G0 with "HeqG") as "-#IH".
+      iApply (wp_mono' with "IH").
+      iIntros (w3 r3 (t3 & e3'')) "!> (#Heq5 & #Heq6)".
+      clear IH1 IH2 IH3.
+      do 2 rewrite wp_bind wp_assert. rewrite wp_pure. predsimpl.
+      iStopProof. pred_unfold. intuition subst; auto.
+
+    - iIntros "#HeqG".
+      rewrite wp_bind wp_pick. predsimpl.
+      iApply (Acc.intro_wp_step t1). iIntros "!> #Heq1".
+      rewrite wp_bind. predsimpl.
+      iPoseProof (IH _ (G0 ,, x∷ṫy.var world.in_zero)) as "IH".
+      rewrite lift_insert. predsimpl.
+      iPoseProof ("IH" with "HeqG Heq1") as "-#IH'"; iClear "IH".
+      iApply (wp_mono' with "IH'").
+      iIntros (w1 θ1 (t2' & e1'')) "!> (#Heq2 & #Heq3)".
+      rewrite wp_pure. predsimpl.
+      iStopProof. pred_unfold. intuition subst; auto.
+
+    - iIntros "#HeqG".
+      rewrite wp_bind. unfold _4.
+      iPoseProof (IH _ (G0 ,, x∷lift t1)) as "IH".
+      rewrite lift_insert. predsimpl.
+      iPoseProof ("IH" with "HeqG") as "-#IH'"; iClear "IH".
+      iApply (wp_mono' with "IH'").
+      iIntros (w1 r1 (t2' & e'')) "!> (#Heq1 & #Heq2)".
+      rewrite wp_pure. predsimpl.
+      iStopProof. pred_unfold. intuition subst; auto.
+
+    - iIntros "#HeqG".
+      rewrite wp_bind. unfold _4.
+      iPoseProof (IH1 _ G0) as "IH"; clear IH1.
+      iPoseProof ("IH" with "HeqG") as "-#IH'"; iClear "IH".
+      iApply (wp_mono' with "IH'").
+      iIntros (w1 r1 (tf & e1'')) "!> (#Heq1 & #Heq2)"; predsimpl.
+
+      rewrite wp_bind. unfold _4.
+      iPoseProof (IH2 w1 G0 with "HeqG") as "-#IH"; clear IH2.
+      iApply (wp_mono' with "IH").
+      iIntros (w2 r2 (t1' & e2'')) "!> (#Heq3 & #Heq4)".
+
+      rewrite wp_bind wp_pick. unfold _4.
+      iApply (Acc.intro_wp_step t2). iIntros "!> #Heq5".
+      rewrite wp_bind wp_assert. unfold _4.
+      rewrite wp_pure. predsimpl.
+      repeat (rewrite ?persist_eq ?persist_lift; predsimpl).
+
+      generalize (@ṫy.var (w2 ▻ world.fresh w2) (world.fresh w2) (@world.in_zero (world.fresh w2) w2)). intros t2'.
+
+      iStopProof. pred_unfold. intuition subst; auto.
+  Qed.
+
+  Lemma generate_complete  {w} (Γ : Ėnv w) (e : Exp) (τ : Ṫy w) (e' : Ėxp w) :
+    Γ |--ₚ e; τ ~> e' ⊢ₚ TPB_algo Γ e τ e'.
+  Proof.
+    pred_unfold. intros ι HT.
+    destruct (generate_complete_aux HT Γ) as [Hcompl].
+    specialize (Hcompl ι (MkEmp _)). pred_unfold.
+    rewrite inst_lift in Hcompl.
+    specialize (Hcompl eq_refl). revert Hcompl.
+    apply wp_mono. intros w1 θ1 [τ1 e1]. cbn.
+    pred_unfold. intuition subst; auto.
+  Qed.
+
+  Lemma generate_correct {w} (Γ : Ėnv w) (e : Exp) (τ : Ṫy w) (e' : Ėxp w) :
+    Γ |--ₚ e; τ ~> e' ⊣⊢ₚ TPB_algo Γ e τ e'.
+  Proof. apply split_bientails; auto using generate_complete, generate_sound. Qed.
+
+End Generator.
