theories/Stlc/MonadFree.v
@@ -1,0 +1,212 @@
+(******************************************************************************)
+(* Copyright (c) 2023 Denis Carnier, Steven Keuchel                           *)
+(* All rights reserved.                                                       *)
+(*                                                                            *)
+(* Redistribution and use in source and binary forms, with or without         *)
+(* modification, are permitted provided that the following conditions are     *)
+(* met:                                                                       *)
+(*                                                                            *)
+(* 1. Redistributions of source code must retain the above copyright notice,  *)
+(*    this list of conditions and the following disclaimer.                   *)
+(*                                                                            *)
+(* 2. Redistributions in binary form must reproduce the above copyright       *)
+(*    notice, this list of conditions and the following disclaimer in the     *)
+(*    documentation and/or other materials provided with the distribution.    *)
+(*                                                                            *)
+(* THIS SOFTWARE IS PROVIDED BY THE COPYRIGHT HOLDERS AND CONTRIBUTORS        *)
+(* "AS IS" AND ANY EXPRESS OR IMPLIED WARRANTIES, INCLUDING, BUT NOT LIMITED  *)
+(* TO, THE IMPLIED WARRANTIES OF MERCHANTABILITY AND FITNESS FOR A PARTICULAR *)
+(* PURPOSE ARE DISCLAIMED. IN NO EVENT SHALL THE COPYRIGHT HOLDER OR          *)
+(* CONTRIBUTORS BE LIABLE FOR ANY DIRECT, INDIRECT, INCIDENTAL, SPECIAL,      *)
+(* EXEMPLARY, OR CONSEQUENTIAL DAMAGES (INCLUDING, BUT NOT LIMITED TO,        *)
+(* PROCUREMENT OF SUBSTITUTE GOODS OR SERVICES; LOSS OF USE, DATA, OR         *)
+(* PROFITS; OR BUSINESS INTERRUPTION) HOWEVER CAUSED AND ON ANY THEORY OF     *)
+(* LIABILITY, WHETHER IN CONTRACT, STRICT LIABILITY, OR TORT (INCLUDING       *)
+(* NEGLIGENCE OR OTHERWISE) ARISING IN ANY WAY OUT OF THE USE OF THIS         *)
+(* SOFTWARE, EVEN IF ADVISED OF THE POSSIBILITY OF SUCH DAMAGE.               *)
+(******************************************************************************)
+
+From Coq Require Import
+  Strings.String.
+From Equations Require Import
+  Equations.
+From iris Require Import
+  proofmode.tactics.
+From Em Require Import
+  Prelude
+  Stlc.Alloc
+  Stlc.Instantiation
+  Stlc.MonadInterface
+  Stlc.Persistence
+  Stlc.Predicates
+  Stlc.Spec
+  Stlc.Substitution
+  Stlc.Worlds.
+
+Import Pred Pred.notations Pred.Acc Sub Pred.proofmode world.notations.
+
+#[local] Set Implicit Arguments.
+
+Inductive Free (A : TYPE) (w : World) : Type :=
+| Ret (a : A w)
+| Fail
+| Assertk (t1 t2 : Ṫy w) (k : Free A w)
+| Choosek α (k : Free A (w ▻ α)).
+#[global] Arguments Ret {A} [w] a.
+#[global] Arguments Fail {A w}.
+#[global] Arguments Choosek {A} [w] α k.
+
+#[export] Instance pure_free : Pure Free :=
+  fun A w a => Ret a.
+
+#[export] Instance bind_free `{reflΘ : Refl Θ, transΘ : Trans Θ, stepΘ : Step Θ} :
+  Bind Θ Free :=
+  fun A B =>
+    fix bind {w} m f {struct m} :=
+    match m with
+    | Ret a           => f _ refl a
+    | Fail            => Fail
+    | Assertk t1 t2 k => Assertk t1 t2 (bind k f)
+    | Choosek α k     => Choosek α (bind k (_4 f step))
+    end.
+
+#[export] Instance tcm_free : TypeCheckM Free :=
+  {| assert w τ1 τ2 := Assertk τ1 τ2 (Ret tt);
+     pick w := let α := world.fresh w in
+               Choosek α (Ret (ṫy.var world.in_zero));
+     fail A w := Fail;
+  |}.
+
+Section Logic.
+
+  Context {Θ} {reflΘ : Refl Θ} {lkreflΘ : LkRefl Θ}
+    {transΘ : Trans Θ} {lktransΘ : LkTrans Θ}
+    {stepΘ : Step Θ} {lkstepΘ : LkStep Θ}
+    {refltransθ : ReflTrans Θ}.
+
+  #[export] Instance wp_free : WeakestPre Θ Free :=
+    fun A =>
+      fix WP (w : World) (m : Free A w) (POST : Box Θ (A ⇢ Pred) w) {struct m} :=
+      match m with
+      | Ret a => POST _ refl a
+      | Fail => ⊥ₚ
+      | Assertk t1 t2 k => t1 =ₚ t2 /\ₚ WP w k POST
+      | Choosek α k =>
+          Acc.wp step (WP (w ▻ α) k (fun w1 r01 => _4 POST step r01))
+      end%P.
+
+  #[export] Instance wlp_free : WeakestLiberalPre Θ Free :=
+    fun A =>
+      fix WLP (w : World) (m : Free A w) (POST : Box Θ (A ⇢ Pred) w) {struct m} :=
+      match m with
+      | Ret a => POST _ refl a
+      | Fail => ⊤ₚ
+      | Assertk t1 t2 k => t1 =ₚ t2 ->ₚ WLP w k POST
+      | Choosek α k =>
+          Acc.wlp step (WLP (w ▻ α) k (fun w1 r01 => _4 POST step r01))
+      end%P.
+
+  Lemma wp_free_mono [A w0] (m : Free A w0) (P Q : Box Θ (A ⇢ Pred) w0) :
+    (∀ w1 (θ : Θ w0 w1) (a : A w1), Acc.wlp θ (P w1 θ a -∗ Q w1 θ a)) ⊢
+    (WP m P -∗ WP m Q).
+  Proof.
+    induction m; cbn; iIntros "#PQ"; unfold _4.
+    - iSpecialize ("PQ" $! w (refl (Refl := reflΘ)) a); auto.
+      now rewrite Acc.wlp_refl.
+    - easy.
+    - iIntros "[#Heq HP]". iSplit; [auto|]. iRevert "HP". now iApply IHm.
+    - iApply Acc.wp_mono. iModIntro. iApply IHm.
+      iIntros (w1 θ1 a1) "!>". rewrite <- persist_pred_trans.
+      rewrite persist_forall. iSpecialize ("PQ" $! w1).
+      rewrite persist_forall. iSpecialize ("PQ" $! (step ⊙ θ1)).
+      rewrite persist_forall. iSpecialize ("PQ" $! a1).
+      Unshelve. all: auto.
+      now rewrite Acc.persist_wlp.
+  Qed.
+
+  Lemma wlp_free_mono [A w0] (m : Free A w0) (P Q : Box Θ (A ⇢ Pred) w0) :
+    (∀ w1 (θ : Θ w0 w1) (a : A w1), Acc.wlp θ (P w1 θ a -∗ Q w1 θ a)) ⊢
+    (WLP m P -∗ WLP m Q).
+  Proof.
+    induction m; cbn; iIntros "#PQ"; unfold _4.
+    - iSpecialize ("PQ" $! w (refl (Refl := reflΘ)) a); auto.
+      now rewrite Acc.wlp_refl.
+    - easy.
+    - iIntros "HP #Heq". rewrite <- wand_is_impl.
+      iSpecialize ("HP" with "Heq"). iRevert "HP". now iApply IHm.
+    - iApply Acc.wlp_mono. iModIntro. iApply IHm.
+      iIntros (w1 θ1 a1) "!>". rewrite <- persist_pred_trans.
+      rewrite persist_forall. iSpecialize ("PQ" $! w1).
+      rewrite persist_forall. iSpecialize ("PQ" $! (step ⊙ θ1)).
+      rewrite persist_forall. iSpecialize ("PQ" $! a1).
+      Unshelve. all: eauto.
+      now rewrite Acc.persist_wlp.
+  Qed.
+
+  Section ProperInstances.
+
+    #[local] Notation "∀ x , P" :=
+    (@forall_relation _ _ (fun x => P%signature))
+      (at level 200, x binder, right associativity) : signature_scope.
+    #[local] Notation "A → P" :=
+      (@pointwise_relation A _ P%signature) : signature_scope.
+
+    #[export] Instance proper_wp_entails {A w} (m : Free A w) :
+      Proper ((∀ w1, Θ w w1 → A w1 → entails) ==> entails) (WP m).
+    Proof.
+      intros P Q PQ. iApply wp_free_mono. iIntros (w1 θ1 a1) "!>".
+      iApply PQ.
+    Qed.
+
+    #[export] Instance proper_wp_bientails {A w} (m : Free A w) :
+      Proper ((∀ w1, Θ w w1 → A w1 → (⊣⊢ₚ)) ==> (⊣⊢ₚ)) (WP m).
+    Proof.
+      intros P Q PQ. unfold pointwise_relation, forall_relation in PQ.
+      apply split_bientails; split; apply proper_wp_entails; intros w1 θ1 a1;
+        specialize (PQ w1 θ1 a1); now apply split_bientails in PQ.
+    Qed.
+
+    #[export] Instance proper_wlp_entails {A w} (m : Free A w) :
+      Proper ((∀ w1, Θ w w1 → A w1 → entails) ==> entails) (WLP m).
+    Proof.
+      intros P Q PQ. iApply wlp_free_mono. iIntros (w1 θ1 a1) "!>".
+      iApply PQ.
+    Qed.
+
+    #[export] Instance proper_wlp_bientails {A w} (m : Free A w):
+      Proper ((∀ w1, Θ w w1 → A w1 → (⊣⊢ₚ)) ==> (⊣⊢ₚ)) (WLP m).
+    Proof.
+      intros P Q PQ. unfold pointwise_relation, forall_relation in PQ.
+      apply split_bientails; split; apply proper_wlp_entails; intros w1 θ1 a1;
+      specialize (PQ w1 θ1 a1); now apply split_bientails in PQ.
+    Qed.
+
+  End ProperInstances.
+
+  #[export] Instance tcmlogic_free : TypeCheckLogicM Θ Free.
+  Proof.
+    constructor; intros; predsimpl; cbn; unfold _4;
+      auto using wp_free_mono, wlp_free_mono.
+    - induction m; cbn; try (firstorder; fail).
+      + apply proper_wp_bientails. intros w1 θ1 b1.
+        now rewrite trans_refl_l.
+      + apply Acc.proper_wp_bientails. rewrite IHm. unfold _4.
+        apply proper_wp_bientails. intros w1 θ1 a1.
+        apply proper_wp_bientails. intros w2 θ2 b2.
+        now rewrite trans_assoc.
+    - induction m; predsimpl; try (firstorder; fail).
+      + apply proper_wlp_bientails. intros w1 θ1 b1. now rewrite trans_refl_l.
+      + rewrite IHm.
+        apply proper_wlp_bientails. intros w1 θ1 a1.
+        apply proper_wlp_bientails. intros w2 θ2 b2.
+        now rewrite trans_assoc.
+    - induction m.
+      + predsimpl.
+      + predsimpl.
+      + predsimpl. now rewrite IHm.
+      + rewrite Acc.wp_impl. apply Acc.proper_wlp_bientails. rewrite IHm.
+        apply proper_wlp_bientails. intros w1 θ1 a1.
+        now rewrite <- persist_pred_trans.
+  Qed.
+
+End Logic.
