theories/Stlc/MonadInterface.v
@@ -1,0 +1,257 @@
+(******************************************************************************)
+(* Copyright (c) 2023 Denis Carnier, Steven Keuchel                           *)
+(* All rights reserved.                                                       *)
+(*                                                                            *)
+(* Redistribution and use in source and binary forms, with or without         *)
+(* modification, are permitted provided that the following conditions are     *)
+(* met:                                                                       *)
+(*                                                                            *)
+(* 1. Redistributions of source code must retain the above copyright notice,  *)
+(*    this list of conditions and the following disclaimer.                   *)
+(*                                                                            *)
+(* 2. Redistributions in binary form must reproduce the above copyright       *)
+(*    notice, this list of conditions and the following disclaimer in the     *)
+(*    documentation and/or other materials provided with the distribution.    *)
+(*                                                                            *)
+(* THIS SOFTWARE IS PROVIDED BY THE COPYRIGHT HOLDERS AND CONTRIBUTORS        *)
+(* "AS IS" AND ANY EXPRESS OR IMPLIED WARRANTIES, INCLUDING, BUT NOT LIMITED  *)
+(* TO, THE IMPLIED WARRANTIES OF MERCHANTABILITY AND FITNESS FOR A PARTICULAR *)
+(* PURPOSE ARE DISCLAIMED. IN NO EVENT SHALL THE COPYRIGHT HOLDER OR          *)
+(* CONTRIBUTORS BE LIABLE FOR ANY DIRECT, INDIRECT, INCIDENTAL, SPECIAL,      *)
+(* EXEMPLARY, OR CONSEQUENTIAL DAMAGES (INCLUDING, BUT NOT LIMITED TO,        *)
+(* PROCUREMENT OF SUBSTITUTE GOODS OR SERVICES; LOSS OF USE, DATA, OR         *)
+(* PROFITS; OR BUSINESS INTERRUPTION) HOWEVER CAUSED AND ON ANY THEORY OF     *)
+(* LIABILITY, WHETHER IN CONTRACT, STRICT LIABILITY, OR TORT (INCLUDING       *)
+(* NEGLIGENCE OR OTHERWISE) ARISING IN ANY WAY OUT OF THE USE OF THIS         *)
+(* SOFTWARE, EVEN IF ADVISED OF THE POSSIBILITY OF SUCH DAMAGE.               *)
+(******************************************************************************)
+
+From Coq Require Import
+  Strings.String.
+From Equations Require Import
+  Equations.
+From stdpp Require Import
+  base gmap.
+From Em Require Import
+  Environment
+  Prelude
+  Stlc.Alloc
+  Stlc.Instantiation
+  Stlc.Persistence
+  Stlc.Predicates
+  Stlc.Sem
+  Stlc.Spec
+  Stlc.Worlds.
+
+Import world.notations.
+Import Pred Pred.notations.
+Import Pred.proofmode.
+Import iris.proofmode.tactics.
+
+#[local] Notation "s [ ζ ]" :=
+  (persist s ζ)
+    (at level 7, left associativity,
+      format "s [ ζ ]").
+#[local] Set Implicit Arguments.
+
+Class Pure (M : TYPE → TYPE) : Type :=
+  pure : ∀ A, ⊧ A ⇢ M A.
+#[global] Arguments pure {M _ A} [w].
+Class Bind (Θ : SUB) (M : TYPE → TYPE) : Type :=
+  bind : ∀ A B, ⊧ M A ⇢ Box Θ (A ⇢ M B) ⇢ M B.
+#[global] Arguments bind {Θ M _ A B} [w].
+
+Module MonadNotations.
+  Notation "' x <- ma ;; mb" :=
+    (bind ma (fun _ _ x => mb))
+      (at level 80, x pattern, ma at next level, mb at level 200, right associativity,
+        format "' x  <-  ma  ;;  mb").
+  Notation "x <- ma ;; mb" :=
+    (bind ma (fun _ _ x => mb))
+      (at level 80, ma at next level, mb at level 200, right associativity).
+
+  Existing Class sub.
+  #[export] Existing Instance trans.
+  #[export] Hint Mode sub - + - : typeclass_instances.
+End MonadNotations.
+
+Class TypeCheckM (M : TYPE -> TYPE) : Type :=
+  { assert   : ⊧ Ṫy ⇢ Ṫy ⇢ M Unit;
+    pick     : ⊧ M Ṫy;
+    fail {A} : ⊧ M A;
+  }.
+#[global] Arguments fail {_ _ _ w}.
+#[global] Arguments pick {_ _ w}.
+
+Class WeakestPre (Θ : SUB) (M : TYPE -> TYPE) : Type :=
+  WP [A] : ⊧ M A ⇢ Box Θ (A ⇢ Pred) ⇢ Pred.
+Class WeakestLiberalPre (Θ : SUB) (M : TYPE -> TYPE) : Type :=
+  WLP [A] : ⊧ M A ⇢ Box Θ (A ⇢ Pred) ⇢ Pred.
+
+Class TypeCheckLogicM
+  Θ {reflΘ : Refl Θ} {stepΘ : Step Θ} {transΘ : Trans Θ}
+  M {pureM : Pure M} {bindM : Bind Θ M} {tcM : TypeCheckM M}
+    {wpM : WeakestPre Θ M} {wlpM : WeakestLiberalPre Θ M} : Type :=
+  { wp_pure [A w] (a : A w) (Q : Box Θ (A ⇢ Pred) w) :
+      WP (pure a) Q ⊣⊢ₚ Q _ refl a;
+    wp_bind [A B w0] (m : M A w0) (f : Box Θ (A ⇢ M B) w0) (Q : Box Θ (B ⇢ Pred) w0) :
+      WP (bind m f) Q ⊣⊢ₚ WP m (fun w1 θ1 a => WP (f _ θ1 a) (_4 Q θ1));
+    wp_assert [w] (σ τ : Ṫy w) (Q : Box Θ (Unit ⇢ Pred) w) :
+      WP (assert σ τ) Q ⊣⊢ₚ σ =ₚ τ /\ₚ Q _ refl tt;
+    wp_pick [w] (Q : Box Θ (Ṫy ⇢ Pred) w) :
+      let α := world.fresh w in
+      WP pick Q ⊣⊢ₚ Acc.wp step (Q (w ▻ α) step (ṫy.var world.in_zero));
+    wp_fail [A w] (Q : Box Θ (A ⇢ Pred) w) :
+      WP fail Q ⊣⊢ₚ ⊥ₚ;
+    wp_mono [A w] (m : M A w) (P Q : Box Θ (A ⇢ Pred) w) :
+      (∀ w1 (θ : Θ w w1) (a : A w1), Acc.wlp θ (P w1 θ a -∗ Q w1 θ a)) ⊢
+      (WP m P -∗ WP m Q);
+
+    wlp_pure [A w] (a : A w) (Q : Box Θ (A ⇢ Pred) w) :
+      WLP (pure a) Q ⊣⊢ₚ Q _ refl a;
+    wlp_bind [A B w0] (m : M A w0) (f : Box Θ (A ⇢ M B) w0) (Q : Box Θ (B ⇢ Pred) w0) :
+      WLP (bind m f) Q ⊣⊢ₚ WLP m (fun w1 θ1 a => WLP (f _ θ1 a) (_4 Q θ1));
+    wlp_assert [w] (σ τ : Ṫy w) (Q : Box Θ (Unit ⇢ Pred) w) :
+      WLP (assert σ τ) Q ⊣⊢ₚ σ =ₚ τ ->ₚ Q _ refl tt;
+    wlp_pick [w] (Q : Box Θ (Ṫy ⇢ Pred) w) :
+      let α := world.fresh w in
+      WLP pick Q ⊣⊢ₚ Acc.wlp step (Q (w ▻ α) step (ṫy.var world.in_zero));
+    wlp_fail [A w] (Q : Box Θ (A ⇢ Pred) w) :
+      WLP fail Q ⊣⊢ₚ ⊤ₚ;
+    wlp_mono [A w] (m : M A w) (P Q : Box Θ (A ⇢ Pred) w) :
+      (∀ w1 (θ : Θ w w1) (a : A w1), Acc.wlp θ (P w1 θ a -∗ Q w1 θ a)) ⊢
+      (WLP m P -∗ WLP m Q);
+
+    wp_impl [A w] (m : M A w) (P : Box Θ (A ⇢ Pred) w) (Q : Pred w) :
+      (WP m P ->ₚ Q) ⊣⊢ₚ WLP m (fun w1 θ1 a1 => P w1 θ1 a1 ->ₚ Q[θ1]);
+  }.
+#[global] Arguments TypeCheckLogicM Θ {_ _ _} _ {_ _ _ _ _}.
+
+Lemma wp_mono' `{TypeCheckLogicM Θ M} {A w} (m : M A w) (P Q : Box Θ (A ⇢ Pred) w) :
+  (WP m P -∗ (∀ₚ w1 θ1 a1, Acc.wlp θ1 (P w1 θ1 a1 -∗ Q w1 θ1 a1)) -∗ WP m Q)%P.
+Proof. iIntros "WP PQ". iRevert "WP". now iApply wp_mono. Qed.
+
+Lemma wlp_mono' `{TypeCheckLogicM Θ M} {A w} (m : M A w) (P Q : Box Θ (A ⇢ Pred) w) :
+  (WLP m P -∗ (∀ₚ w1 θ1 a1, Acc.wlp θ1 (P w1 θ1 a1 -∗ Q w1 θ1 a1)) -∗ WLP m Q)%P.
+Proof. iIntros "WP PQ". iRevert "WP". now iApply wlp_mono. Qed.
+
+Definition wp_diamond {Θ : SUB} {A} :
+  ⊧ Diamond Θ A ⇢ Box Θ (A ⇢ Pred) ⇢ Pred :=
+  fun w '(existT w1 (θ, a)) Q => Acc.wp θ (Q w1 θ a).
+
+Definition wlp_diamond {Θ : SUB} {A} :
+  ⊧ Diamond Θ A ⇢ Box Θ (A ⇢ Pred) ⇢ Pred :=
+  fun w '(existT w1 (θ, a)) Q => Acc.wlp θ (Q w1 θ a).
+
+Definition wp_option {A w1 w2} :
+  Option A w1 -> (A w1 -> Pred w2) -> Pred w2 :=
+  fun o Q =>
+    match o with
+    | Some a => Q a
+    | None => ⊥ₚ
+    end%P.
+
+Definition wlp_option {A w1 w2} :
+  Option A w1 -> (A w1 -> Pred w2) -> Pred w2 :=
+  fun o Q =>
+    match o with
+    | Some a => Q a
+    | None => ⊤ₚ
+    end%P.
+
+Section OptionDiamond.
+
+  Definition OptionDiamond (Θ : SUB) (A : TYPE) : TYPE :=
+    Option (Diamond Θ A).
+
+  #[export] Instance wp_optiondiamond {Θ : SUB} : WeakestPre Θ (OptionDiamond Θ) :=
+    fun A w m Q => wp_option m (fun d => wp_diamond d Q).
+  #[global] Arguments wp_optiondiamond {Θ} {A}%indexed_scope [w] _ _%B _.
+  #[global] Instance params_wp_optiondiamond : Params (@wp_optiondiamond) 5 := {}.
+
+  #[export] Instance proper_wp_optiondiamond_bientails {Θ A w} :
+    Proper
+      (pointwise_relation _
+         (forall_relation
+            (fun _ => pointwise_relation _
+                        (pointwise_relation _ (⊣⊢ₚ))) ==> (⊣⊢ₚ)))
+      (@wp_optiondiamond Θ A w).
+  Proof.
+    intros d p q pq. destruct d as [(w1 & r01 & a)|]; cbn; [|easy].
+    apply Acc.proper_wp_bientails. apply pq.
+  Qed.
+
+  #[export] Instance proper_wp_optiondiamond_entails {Θ A w} :
+    Proper
+      (pointwise_relation _
+         (forall_relation
+            (fun _ => pointwise_relation _
+                        (pointwise_relation _ entails)) ==> entails))
+      (@wp_optiondiamond Θ A w).
+  Proof.
+    intros d p q pq. destruct d as [(w1 & r01 & a)|]; cbn; [|easy].
+    apply Acc.proper_wp_entails. apply pq.
+  Qed.
+
+  Lemma wp_optiondiamond_and {Θ A w} (d : OptionDiamond Θ A w)
+    (P : Box Θ (A ⇢ Pred) w) (Q : Pred w) :
+    WP d P /\ₚ Q ⊣⊢ₚ WP d (fun w1 θ1 a1 => P w1 θ1 a1 /\ₚ persist Q θ1).
+  Proof.
+    destruct d as [(w1 & θ1 & a1)|]; cbn.
+    - now rewrite Acc.and_wp_l.
+    - now rewrite bi.False_and.
+  Qed.
+
+  Lemma wp_optiondiamond_monotonic' {Θ A w} (d : OptionDiamond Θ A w)
+    (R : Pred w) (P Q : Box Θ (A ⇢ Pred) w) :
+    (forall w1 (r : Θ w w1) (a : A w1),
+        persist R r ⊢ₚ P w1 r a ->ₚ Q w1 r a) ->
+    R ⊢ₚ WP d P ->ₚ WP d Q.
+  Proof.
+    intros pq. destruct d as [(w1 & r01 & a)|]; cbn.
+    - specialize (pq w1 r01 a).
+      apply impl_and_adjoint.
+      rewrite Acc.and_wp_r.
+      apply Acc.proper_wp_entails.
+      apply impl_and_adjoint.
+      apply pq.
+    - apply impl_and_adjoint.
+      now rewrite and_false_r.
+  Qed.
+
+  #[export] Instance pure_optiondiaomd {Θ} {reflΘ : Refl Θ} :
+    Pure (OptionDiamond Θ) :=
+    fun A w a => Some (existT w (refl, a)).
+
+  #[export] Instance bind_optiondiamond {Θ} {transΘ : Trans Θ} :
+    Bind Θ (OptionDiamond Θ) :=
+    fun A B w m f =>
+      option.bind m
+        (fun '(existT w1 (θ1,a1)) =>
+           option.bind (f w1 θ1 a1)
+             (fun '(existT w2 (θ2,b2)) =>
+                Some (existT w2 (trans θ1 θ2, b2)))).
+
+  (* Lemma wp_optiondiamond_pure {Θ} {reflΘ : Refl Θ} {lkreflΘ : LkRefl Θ} *)
+  (*   {A w0} (a : A w0) (Q : Box Θ (A ⇢ Pred) w0) : *)
+  (*   wp_optiondiamond (pure (M := DiamondT Θ Option) a) Q ⊣⊢ₚ Q _ refl a. *)
+  (* Proof. cbn. now rewrite Acc.wp_refl. Qed. *)
+
+  Lemma wp_optiondiamond_bind {Θ} {transΘ : Trans Θ} {lkTransΘ : LkTrans Θ}
+    {A B w0} (d : OptionDiamond Θ A w0) (f : Box Θ (A ⇢ OptionDiamond Θ B) w0)
+    (Q : Box Θ (B  ⇢ Pred) w0) :
+    WP (bind d f) Q ⊣⊢ₚ WP d (fun w1 ζ1 a1 => WP (f w1 ζ1 a1) (_4 Q ζ1)).
+  Proof.
+    destruct d as [(w1 & r01 & a)|]; cbn; [|reflexivity].
+    destruct (f w1 r01 a) as [(w2 & r12 & b2)|]; cbn;
+      now rewrite ?Acc.wp_trans ?Acc.wp_false.
+  Qed.
+
+End OptionDiamond.
+
+#[local] Instance instpred_diamond {Θ A} `{ipA : InstPred A} :
+  InstPred (Diamond Θ A) :=
+  fun w m => wp_diamond m (fun _ _ a => instpred a).
+#[export] Instance instpred_optiondiamond {Θ A} `{ipA : InstPred A} :
+  InstPred (OptionDiamond Θ A) :=
+  fun w m => WP m (fun _ _ a => instpred a).
