theories/Stlc/MonadPrenex.v
@@ -1,0 +1,106 @@
+(******************************************************************************)
+(* Copyright (c) 2023 Denis Carnier, Steven Keuchel                           *)
+(* All rights reserved.                                                       *)
+(*                                                                            *)
+(* Redistribution and use in source and binary forms, with or without         *)
+(* modification, are permitted provided that the following conditions are     *)
+(* met:                                                                       *)
+(*                                                                            *)
+(* 1. Redistributions of source code must retain the above copyright notice,  *)
+(*    this list of conditions and the following disclaimer.                   *)
+(*                                                                            *)
+(* 2. Redistributions in binary form must reproduce the above copyright       *)
+(*    notice, this list of conditions and the following disclaimer in the     *)
+(*    documentation and/or other materials provided with the distribution.    *)
+(*                                                                            *)
+(* THIS SOFTWARE IS PROVIDED BY THE COPYRIGHT HOLDERS AND CONTRIBUTORS        *)
+(* "AS IS" AND ANY EXPRESS OR IMPLIED WARRANTIES, INCLUDING, BUT NOT LIMITED  *)
+(* TO, THE IMPLIED WARRANTIES OF MERCHANTABILITY AND FITNESS FOR A PARTICULAR *)
+(* PURPOSE ARE DISCLAIMED. IN NO EVENT SHALL THE COPYRIGHT HOLDER OR          *)
+(* CONTRIBUTORS BE LIABLE FOR ANY DIRECT, INDIRECT, INCIDENTAL, SPECIAL,      *)
+(* EXEMPLARY, OR CONSEQUENTIAL DAMAGES (INCLUDING, BUT NOT LIMITED TO,        *)
+(* PROCUREMENT OF SUBSTITUTE GOODS OR SERVICES; LOSS OF USE, DATA, OR         *)
+(* PROFITS; OR BUSINESS INTERRUPTION) HOWEVER CAUSED AND ON ANY THEORY OF     *)
+(* LIABILITY, WHETHER IN CONTRACT, STRICT LIABILITY, OR TORT (INCLUDING       *)
+(* NEGLIGENCE OR OTHERWISE) ARISING IN ANY WAY OUT OF THE USE OF THIS         *)
+(* SOFTWARE, EVEN IF ADVISED OF THE POSSIBILITY OF SUCH DAMAGE.               *)
+(******************************************************************************)
+
+From iris Require Import
+  proofmode.tactics.
+From Em Require Import
+  Prelude
+  Stlc.Alloc
+  Stlc.MonadInterface
+  Stlc.Instantiation
+  Stlc.Persistence
+  Stlc.Predicates
+  Stlc.Spec
+  Stlc.Worlds.
+
+Import MonadNotations Pred Pred.Acc Pred.notations Pred.proofmode
+  world.notations.
+
+#[local] Set Implicit Arguments.
+
+Definition Prenex A := Option ◇⁺(List (Ṫy * Ṫy) * A).
+
+#[export] Instance pure_prenex : Pure Prenex :=
+  fun A w a => Some (existT w (refl, (List.nil, a))).
+#[export] Instance bind_prenex : Bind Alloc Prenex :=
+  fun A B w (m : OptionDiamond Alloc (List (Ṫy * Ṫy) * A) w)
+      (f : Box Alloc (A ⇢ OptionDiamond Alloc (List (Ṫy * Ṫy) * B)) w) =>
+    '(C1,a1) <- m ;;
+    '(C2,b2) <- f _ _ a1 ;;
+    pure (persist C1 _ ++ C2, b2).
+#[export] Instance tcm_prenex : TypeCheckM Prenex :=
+  {| assert w τ1 τ2 := Some (existT w (refl, ([(τ1,τ2)], tt)));
+     pick w := let α := world.fresh w in
+               Some (existT (w ▻ α) (step, (List.nil, ṫy.var world.in_zero)));
+     fail A w := None;
+  |}.
+
+#[local] Existing Instance instpred_prod_ty.
+#[local] Existing Instance instpred_persist_prod_ty.
+
+#[export] Instance wp_prenex : WeakestPre Alloc Prenex :=
+  fun A w o Q =>
+    wp_option o
+      (fun d =>
+         wp_diamond d
+           (fun w1 θ1 '(C,a) => instpred C /\ₚ Q w1 θ1 a))%P.
+
+#[export] Instance wlp_prenex : WeakestLiberalPre Alloc Prenex :=
+  fun A w o Q =>
+    wlp_option o
+      (fun d =>
+         wlp_diamond d
+           (fun w1 θ1 '(C,a) => instpred C ->ₚ Q w1 θ1 a))%P.
+
+
+#[export] Instance tcmlogic_prenex : TypeCheckLogicM Alloc Prenex.
+Proof.
+  constructor; intros; predsimpl.
+  - destruct m as [(w1 & θ1 & C1 & a1)|]; predsimpl.
+    destruct f as [(w2 & θ2 & C2 & b2)|]; predsimpl.
+    rewrite Acc.and_wp_r. apply Acc.proper_wp_bientails.
+    rewrite bi.and_assoc. apply bi.and_proper; auto.
+    rewrite instpred_list_app. apply bi.and_proper; auto.
+    now rewrite instpred_persist.
+  - destruct m as [(w1 & θ1 & C1 & a1)|]; predsimpl.
+    iIntros "PQ". iApply Acc.wp_mono. iPoseProof ("PQ" $! w1 θ1 a1) as "PQ".
+    iIntros "!> [HC HP]". rewrite Acc.persist_wlp.
+    iSplit; auto. iApply "PQ"; auto.
+  - destruct m as [(w1 & θ1 & C1 & a1)|]; predsimpl.
+    destruct f as [(w2 & θ2 & C2 & b2)|]; predsimpl.
+    rewrite Acc.wlp_frame. apply Acc.proper_wlp_bientails.
+    rewrite <- impl_and. apply bi.impl_proper; auto.
+    rewrite instpred_list_app. apply bi.and_proper; auto.
+    now rewrite instpred_persist_list.
+  - destruct m as [(w1 & θ1 & C1 & a1)|]; predsimpl.
+    iIntros "PQ". iApply Acc.wlp_mono. iPoseProof ("PQ" $! w1 θ1 a1) as "PQ".
+    iIntros "!> CP C". rewrite Acc.persist_wlp -wand_is_impl.
+    iApply "PQ". by iApply "CP".
+  - destruct m as [(w1 & θ1 & C1 & a1)|]; predsimpl.
+    rewrite Acc.wp_impl. predsimpl.
+Qed.
