Makefile
@@ -1,19 +1,34 @@
 # Always run with nproc jobs by default. Can be overridden by the user.
 MAKEFLAGS := --jobs=$(shell nproc)
 
-all: Makefile.coq
-	@+$(MAKE) -f Makefile.coq all
+# Comment out the below line if you want to be quiet by default.
+VERBOSE ?= 1
+ifeq ($(V),1)
+E=@true
+Q=
+else
+E=@echo
+Q=@
+MAKEFLAGS += -s
+endif
+
+SRCS := $(shell egrep '^.*\.v$$' _CoqProject | grep -v '^#')
+AUXS := $(join $(dir $(SRCS)), $(addprefix ., $(notdir $(SRCS:.v=.aux))))
+
+.PHONY: coq clean summaxlen install uninstall pretty-timed make-pretty-timed-before make-pretty-timed-after print-pretty-timed-diff
+
+coq: Makefile.coq
+	$(E) "MAKE Makefile.coq"
+	$(Q)$(MAKE) -f Makefile.coq
+
+Makefile.coq: _CoqProject Makefile $(SRCS)
+	$(E) "COQ_MAKEFILE Makefile.coq"
+	$(Q)coq_makefile -f _CoqProject -o Makefile.coq
 
 clean: Makefile.coq
-	@+$(MAKE) -f Makefile.coq cleanall
-	@rm -f Makefile.coq Makefile.coq.conf
+	$(Q)$(MAKE) -f Makefile.coq clean
+	$(Q)rm -f $(AUXS)
+	$(Q)rm -f Makefile.coq *.bak *.d *.glob *~ result*
 
-Makefile.coq: _CoqProject
-	$(COQBIN)coq_makefile -f _CoqProject -o Makefile.coq
-
-force _CoqProject Makefile: ;
-
-%: Makefile.coq force
-	@+$(MAKE) -f Makefile.coq $@
-
-.PHONY: all clean force
+install uninstall pretty-timed make-pretty-timed-before make-pretty-timed-after print-pretty-timed-diff: Makefile.coq
+	$(Q)$(MAKE) -f Makefile.coq $@
